full proof of ChaCha20 savx2

proof/crypto_stream/chacha20/ref/ChaCha20_savx2_proof.ec
@@ -5,1000 +5,6 @@ require import ChaCha20_Spec ChaCha20_pref ChaCha20_pref_proof ChaCha20_sref_pro
 require import StdRing StdOrder.
 import IntOrder.
 
-op x8 (k1 k2 k3 k4 k5 k6 k7 k8: W32.t Array16.t) =
-  Array16.init (fun i => W8u32.pack8 [k1.[i]; k2.[i]; k3.[i]; k4.[i]; k5.[i]; k6.[i]; k7.[i]; k8.[i]]).
-(*
-  Array16.of_list W256.zero [
-     W8u32.pack8 [k1.[0 ]; k2.[0 ]; k3.[0 ]; k4.[0 ]; k5.[0 ]; k6.[0 ]; k7.[0 ]; k8.[0 ]];
-     W8u32.pack8 [k1.[1 ]; k2.[1 ]; k3.[1 ]; k4.[1 ]; k5.[1 ]; k6.[1 ]; k7.[1 ]; k8.[1 ]];
-     W8u32.pack8 [k1.[2 ]; k2.[2 ]; k3.[2 ]; k4.[2 ]; k5.[2 ]; k6.[2 ]; k7.[2 ]; k8.[2 ]];
-     W8u32.pack8 [k1.[3 ]; k2.[3 ]; k3.[3 ]; k4.[3 ]; k5.[3 ]; k6.[3 ]; k7.[3 ]; k8.[3 ]];
-     W8u32.pack8 [k1.[4 ]; k2.[4 ]; k3.[4 ]; k4.[4 ]; k5.[4 ]; k6.[4 ]; k7.[4 ]; k8.[4 ]];
-     W8u32.pack8 [k1.[5 ]; k2.[5 ]; k3.[5 ]; k4.[5 ]; k5.[5 ]; k6.[5 ]; k7.[5 ]; k8.[5 ]];
-     W8u32.pack8 [k1.[6 ]; k2.[6 ]; k3.[6 ]; k4.[6 ]; k5.[6 ]; k6.[6 ]; k7.[6 ]; k8.[6 ]];
-     W8u32.pack8 [k1.[7 ]; k2.[7 ]; k3.[7 ]; k4.[7 ]; k5.[7 ]; k6.[7 ]; k7.[7 ]; k8.[7 ]];
-     W8u32.pack8 [k1.[8 ]; k2.[8 ]; k3.[8 ]; k4.[8 ]; k5.[8 ]; k6.[8 ]; k7.[8 ]; k8.[8 ]];
-     W8u32.pack8 [k1.[9 ]; k2.[9 ]; k3.[9 ]; k4.[9 ]; k5.[9 ]; k6.[9 ]; k7.[9 ]; k8.[9 ]];
-     W8u32.pack8 [k1.[10]; k2.[10]; k3.[10]; k4.[10]; k5.[10]; k6.[10]; k7.[10]; k8.[10]];
-     W8u32.pack8 [k1.[11]; k2.[11]; k3.[11]; k4.[11]; k5.[11]; k6.[11]; k7.[11]; k8.[11]];
-     W8u32.pack8 [k1.[12]; k2.[12]; k3.[12]; k4.[12]; k5.[12]; k6.[12]; k7.[12]; k8.[12]];
-     W8u32.pack8 [k1.[13]; k2.[13]; k3.[13]; k4.[13]; k5.[13]; k6.[13]; k7.[13]; k8.[13]];
-     W8u32.pack8 [k1.[14]; k2.[14]; k3.[14]; k4.[14]; k5.[14]; k6.[14]; k7.[14]; k8.[14]];
-     W8u32.pack8 [k1.[15]; k2.[15]; k3.[15]; k4.[15]; k5.[15]; k6.[15]; k7.[15]; k8.[15]]
-  ].
-*)
-
-lemma get_x8 (k1 k2 k3 k4 k5 k6 k7 k8: W32.t Array16.t) i: 
-  0 <= i < 16 => 
-  (x8 k1 k2 k3 k4 k5 k6 k7 k8).[i] = 
-     W8u32.pack8 [k1.[i]; k2.[i]; k3.[i]; k4.[i]; k5.[i]; k6.[i]; k7.[i]; k8.[i]].
-proof.
-  by move => h; rewrite /x8 initE h.
-qed.
-
-lemma set_x8 (k1 k2 k3 k4 k5 k6 k7 k8: W32.t Array16.t) i w1 w2 w3 w4 w5 w6 w7 w8: 
-  0 <= i < 16 =>
-  (x8 k1 k2 k3 k4 k5 k6 k7 k8).[i <- W8u32.pack8 [w1;w2;w3;w4;w5;w6;w7;w8]] =
-  x8 k1.[i<-w1] k2.[i<-w2] k3.[i<-w3] k4.[i<-w4] k5.[i<-w5] k6.[i<-w6] k7.[i<-w7] k8.[i<-w8].
-proof.
-  move=> hi; apply Array16.ext_eq => j hj.  
-  rewrite /x8 setE 2!initE hj /= initE hj /= !Array16.get_set_if hi /=.
-  by case: (j = i).
-qed.
-
-(* Move this *)
-lemma x86_8u32_rol_xor r w : 0 < r < 32 => 
-  x86_VPSLL_8u32 w (W8.of_int r) `^` x86_VPSRL_8u32 w (W8.of_int (32 - r))  =
-  map (transpose W32.rol r) w.
-proof.
-  move=> hr;rewrite /x86_VPSRL_8u32 /x86_VPSLL_8u32 /(`>>`) /(`<<`).
-  rewrite !W8.to_uint_small /= 1,2:/# /=.
-  rewrite /map; congr; apply W8u32.Pack.ext_eq => j hj.
-  by rewrite map2iE 1:// 3!initE hj /= W32.rol_xor 1:/# 2?modz_small 1,2:/#.
-qed.
-
-phoare rotate_x8_s k0 i0 r0 : 
-  [M.rotate_x8_s : 
-    k = k0 /\ i = i0 /\ r = r0 /\ 0 <= i < 16 /\ 0 < r < 32 /\ r16 = g_r16 /\ r8 = g_r8 
-    ==>
-    res = k0.[i0 <- W8u32.pack8_t (W8u32.Pack.map (fun (x:W32.t) => rol x r0) (W8u32.unpack32 k0.[i0]))]] = 1%r.
-proof.
-  proc => /=.
-  if; 1: by wp;skip.  
-  if; 1: by wp;skip.
-  wp;skip => /> &m hi1 hi2 hr1 hr2 _ _; congr.
-  by rewrite W256.xorwC get_setE 1:// /= x86_8u32_rol_xor.
-qed.
-
-equiv eq_line_x8_v_ a_ c_ k_ : ChaCha20_pavx2.M.line_x1_8 ~ M._line_x8_v :
-  ={a,b,c,r} /\ k{2} = k_ /\ a{1} = a_ /\ c{1} = c_ /\
-   k{2} = (x8 k1 k2 k3 k4 k5 k6 k7 k8){1} /\ 
-   0 <= a{1} < 16 /\ 0 <= b{1} < 16 /\ 0 <= c{1} < 16 /\ 0 < r{1} < 32 /\
-   r16{2} = g_r16 /\ r8{2} = g_r8 
-  ==> 
-  res{2} = x8 res{1}.`1 res{1}.`2 res{1}.`3 res{1}.`4 res{1}.`5 res{1}.`6 res{1}.`7 res{1}.`8 /\
-  forall i, 0 <= i < 16 => i <> a_ => i <> c_ => res{2}.[i] = k_.[i].
-proof.
-  proc => /=.
-  inline{1} ChaCha20_pref.M.line.
-  interleave{1} [2:4] [11:4] [20:4] [29:4] [38:4] [47:4] [56:4] [65:4] 1.
-  swap{1} 1 32.
-  interleave{1} [33:1] [38:1] [43:1] [48:1] [53:1] [58:1] [63:1] [68:1] 5.
-  sp 32 0.
-  seq 16 1 : (#{/~k{2}}pre /\ k{2} = (x8 k k0 k9 k10 k11 k12 k13 k14){1} /\
-                forall i, 0 <= i < 16 => i <> a_ => i <> c_ => k{2}.[i] = k_.[i]).
-  + wp;skip => /> &1 &2 ha1 ha2 hb1 hb2 hc1 hc2 hr1 hr2.
-    split; 1: by rewrite /x86_VPADD_8u32 !get_x8 1,2:// -set_x8.
-    by move=> ??? h ?;rewrite Array16.get_setE // h.
-  seq 8 1 : (#pre). 
-  + wp;skip => /> &1 &2 ha1 ha2 hb1 hb2 hc1 hc2 hr1 hr2 hi.
-    split; 1: by rewrite !get_x8 1,2:// -set_x8.
-    by move=> ???? h;rewrite Array16.get_setE // h /= hi.
-  wp;ecall{2} (rotate_x8_s k{2} c{2} r{2}); skip => /> &1 &2 ha1 ha2 hb1 hb2 hc1 hc2 hr1 hr2 hi.
-  split; 1: by rewrite !get_x8 1,2:// -set_x8.
-  by move=> ???? h;rewrite Array16.get_setE // h /= hi.
-qed.
-
-equiv eq_line_2 a0_ c0_ a1_ c1_ k_ :  ChaCha20_pavx2.M.line_2_x1_8 ~ M.line_x8_v : 
-  ={a0,b0,c0,r0,a1,b1,c1,r1} /\ k{2} = k_ /\ a0{1} = a0_ /\ c0{1} = c0_ /\ a1{1} = a1_ /\ c1{1} = c1_ /\
-   k{2} = (x8 k1 k2 k3 k4 k5 k6 k7 k8){1} /\ 
-   0 <= a0{1} < 16 /\ 0 <= b0{1} < 16 /\ 0 <= c0{1} < 16 /\ 0 < r0{1} < 32 /\
-   0 <= a1{1} < 16 /\ 0 <= b1{1} < 16 /\ 0 <= c1{1} < 16 /\ 0 < r1{1} < 32 /\
-   r16{2} = g_r16 /\ r8{2} = g_r8 
-  ==> 
-  res{2} = x8 res{1}.`1 res{1}.`2 res{1}.`3 res{1}.`4 res{1}.`5 res{1}.`6 res{1}.`7 res{1}.`8 /\
-  forall i, 0 <= i < 16 => i <> a0_ => i <> c0_ => i <> a1_ => i <> c1_ => res{2}.[i] = k_.[i].
-proof.
-  proc => /=.
-  inline{1} ChaCha20_pavx2.M.line_2.
-  interleave{1} [2:8] [18:8] [34:8] [50:8] [66:8] [82:8] [98:8] [114:8] 1.
-  swap{1} 1 64.
-  interleave{1} [65:1] [73:1] [81:1] [89:1] [97:1] [105:1] [113:1] [121:1] 8.
-  sp 64 0.
-  seq 16 1 : (#{/~k{2}}pre /\ k{2} = (x8 k k0 k9 k10 k11 k12 k13 k14){1} /\
-     forall i, 0 <= i < 16 => i <> a0_ => i <> c0_ => i <> a1_ => i <> c1_ => k{2}.[i] = k_.[i]).
-  + wp;skip => /> &1 &2 ha1 ha2 hb1 hb2 hc1 hc2 hd1 hd2 ha1' ha2' hb1' hb2' hc1' hc2' hd1' hd2'.
-    split; 1: by rewrite /x86_VPADD_8u32 !get_x8 1,2:// -set_x8.
-    by move=> ??? h *;rewrite Array16.get_setE // h.
-  seq 8 1 : (#pre).
-  + wp;skip => /> &1 &2 ha1 ha2 hb1 hb2 hc1 hc2 hd1 hd2 ha1' ha2' hb1' hb2' hc1' hc2' hd1' hd2' hi.
-    split; 1: by rewrite /x86_VPADD_8u32 !get_x8 1,2:// -set_x8. 
-    by move=> ????? h *;rewrite Array16.get_setE // h /= hi.
-  seq 8 1 : (#pre). 
-  + wp;skip => /> &1 &2 ha1 ha2 hb1 hb2 hc1 hc2 hd1 hd2 ha1' ha2' hb1' hb2' hc1' hc2' hd1' hd2' hi.
-    split; 1: by rewrite !get_x8 1,2:// -set_x8.
-    by move=> ???? h *;rewrite Array16.get_setE // h /= hi.
-  seq 8 1 : (#pre). 
-  + wp;skip => /> &1 &2 ha1 ha2 hb1 hb2 hc1 hc2 hd1 hd2 ha1' ha2' hb1' hb2' hc1' hc2' hd1' hd2' hi.
-    split; 1: by rewrite !get_x8 1,2:// -set_x8.
-    by move=> ?????? h;rewrite Array16.get_setE // h /= hi.
-  seq 8 1 : (#pre).
-  + wp; ecall{2} (rotate_x8_s k{2} c0{2} r0{2}); skip => /> 
-      &1 &2 ha1 ha2 hb1 hb2 hc1 hc2 hd1 hd2 ha1' ha2' hb1' hb2' hc1' hc2' hd1' hd2' hi.
-    split; 1: by rewrite !get_x8 1,2:// -set_x8.
-    by move=> ???? h *;rewrite Array16.get_setE // h /= hi.
-  wp; ecall{2} (rotate_x8_s k{2} c1{2} r1{2}); skip => /> 
-    &1 &2 ha1 ha2 hb1 hb2 hc1 hc2 hd1 hd2 ha1' ha2' hb1' hb2' hc1' hc2' hd1' hd2' hi.
-  split; 1: by rewrite !get_x8 1,2:// -set_x8.
-  by move=> ?????? h;rewrite Array16.get_setE // h /= hi.
-qed.
-
-equiv eq_double_quarter_round_x8 a0_ b0_ c0_ d0_ a1_ b1_ c1_ d1_ k_ : 
-    ChaCha20_pavx2.M.double_quarter_round_x8 ~ 
-    ChaCha20_savx2.M.double_quarter_round_x8: 
-    ={a0,b0,c0,d0,a1,b1,c1,d1} /\
-     k{2} = k_ /\ a0{1} = a0_ /\ b0{1} = b0_ /\ c0{1} = c0_ /\ d0{1} = d0_ /\
-                  a1{1} = a1_ /\ b1{1} = b1_ /\ c1{1} = c1_ /\ d1{1} = d1_ /\ 
-     k{2} = (x8 k1 k2 k3 k4 k5 k6 k7 k8){1}  /\ 
-     0 <= a0{1} < 16 /\ 0 <= b0{1} < 16 /\ 0 <= c0{1} < 16 /\ 0 <= d0{1} < 16  /\
-     0 <= a1{1} < 16 /\ 0 <= b1{1} < 16 /\ 0 <= c1{1} < 16 /\ 0 <= d1{1} < 16  /\
-     r16{2} = g_r16 /\ r8{2} = g_r8 
-    ==> 
-    res{2} = x8 res{1}.`1 res{1}.`2 res{1}.`3 res{1}.`4 res{1}.`5 res{1}.`6 res{1}.`7 res{1}.`8 /\
-     forall i, 0 <= i < 16 => i <> a0_ => i <> b0_ => i <> c0_ => i <> d0_ =>
-                             i <> a1_ => i <> b1_ => i <> c1_ => i <> d1_ =>
-               res{2}.[i] = k_.[i].
-proof.
-  proc => /=; wp.
-  ecall (eq_line_x8_v_ c1_ b1_ k{2})=> /=.
-  ecall (eq_line_2 c0_ b0_ a1_ d1_ k{2})=> /=.
-  ecall (eq_line_2 a0_ d0_ c1_ b1_ k{2})=> /=.
-  ecall (eq_line_2 c0_ b0_ a1_ d1_ k{2})=> /=.
-  ecall (eq_line_x8_v_ a0_ d0_ k{2})=> /=; skip => /> /#.
-qed.
-
-equiv eq_column_round_x8 : ChaCha20_pavx2.M.column_round_x8 ~ ChaCha20_savx2.M.column_round_x8 : 
-  k{2} = (x8 k1 k2 k3 k4 k5 k6 k7 k8){1}  /\
-   k15{2} = k{2}.[15] /\ s_r16{2} = g_r16 /\ s_r8{2} = g_r8 
-  ==> 
-  res{2}.`1 = x8 res{1}.`1 res{1}.`2 res{1}.`3 res{1}.`4 res{1}.`5 res{1}.`6 res{1}.`7 res{1}.`8 /\
-   res{2}.`2 = res{2}.`1.[14].
-proof.
-  proc => /=; wp.
-  ecall (eq_double_quarter_round_x8 1 5 9 13 3 7 11 15 k{2}); wp => /=.
-  ecall (eq_double_quarter_round_x8 0 4 8 12 2 6 10 14 k{2}); wp => /=.
-  skip => /> &1 r1 hi.
-  by rewrite -(hi 15) // Array16.set_notmod /= => r2 ->. 
-qed.
-
-equiv eq_diagonal_round_x8 : ChaCha20_pavx2.M.diagonal_round_x8 ~ ChaCha20_savx2.M.diagonal_round_x8 : 
-  k{2} = (x8 k1 k2 k3 k4 k5 k6 k7 k8){1}  /\
-   k14{2} = k{2}.[14] /\ s_r16{2} = g_r16 /\ s_r8{2} = g_r8 
-  ==> 
-  res{2}.`1 = x8 res{1}.`1 res{1}.`2 res{1}.`3 res{1}.`4 res{1}.`5 res{1}.`6 res{1}.`7 res{1}.`8 /\
-   res{2}.`2 = res{2}.`1.[15].
-proof.
-  proc => /=; wp.
-  ecall (eq_double_quarter_round_x8 2 7 8 13 3 4 9 14 k{2}); wp => /=.
-  ecall (eq_double_quarter_round_x8 1 6 11 12 0 5 10 15 k{2}); wp => /=.
-  skip => /> &1 r1 hi.
-  by rewrite -(hi 14) // Array16.set_notmod /= => r2 ->. 
-qed.
-
-equiv eq_rounds_x8 : ChaCha20_pavx2.M.rounds_x8 ~ ChaCha20_savx2.M.rounds_x8 :
-  k{2} = (x8 k1 k2 k3 k4 k5 k6 k7 k8){1} /\ s_r16{2} = g_r16 /\ s_r8{2} = g_r8 
-  ==> 
-  res{2} = x8 res{1}.`1 res{1}.`2 res{1}.`3 res{1}.`4 res{1}.`5 res{1}.`6 res{1}.`7 res{1}.`8.
-proof.
-  proc => /=; wp.
-  while (#pre /\ c{1} = W64.to_uint c{2} /\ (k15 = k.[15]){2}).
-  + wp; call eq_diagonal_round_x8; call eq_column_round_x8; skip => /> *.
-    rewrite ultE /=;rewrite to_uintD_small //= 1:/#.
-  by wp; skip => /> *;rewrite Array16.set_notmod.
-qed.
- 
-equiv eq_init_x8 : ChaCha20_pavx2.M.init_x8 ~ M.init_x8 : 
-  key{1} = to_uint key{2} /\ nonce{1} = to_uint nonce{2} /\ ={counter,Glob.mem} /\
-  (key + 32 < W64.modulus /\ nonce + 12 < W64.modulus){1} 
-  ==>
-  res{2} = x8 res{1}.`1 res{1}.`2 res{1}.`3 res{1}.`4 res{1}.`5 res{1}.`6 res{1}.`7 res{1}.`8.
-proof.
-  proc => /=.
-  inline ChaCha20_pref.M.init.
-  do 2! unroll for{1} ^while; do 2! unroll for{2} ^while.
-  conseq (_ : Array16.all_eq st_{2} (x8 st1{1} st2{1} st3{1} st4{1} st5{1} st6{1} st7{1} st8{1})).
-  + by move=> *; apply Array16.all_eq_eq.
-  wp; skip; cbv delta => /> &2 h1 h2.
-  have -> /= : to_uint (key{2} + W64.of_int 4) = to_uint key{2} + 4.
-  + by rewrite W64.to_uintD_small //= /#.
-  have -> /= : to_uint (key{2} + W64.of_int 8) = to_uint key{2} + 8.  
-  + by rewrite W64.to_uintD_small //= /#.
-  have -> /= : to_uint (key{2} + W64.of_int 12) = to_uint key{2} + 12.  
-  + by rewrite W64.to_uintD_small //= /#.
-  have -> /= : to_uint (key{2} + W64.of_int 16) = to_uint key{2} + 16.  
-  + by rewrite W64.to_uintD_small //= /#.
-  have -> /= : to_uint (key{2} + W64.of_int 20) = to_uint key{2} + 20.  
-  + by rewrite W64.to_uintD_small //= /#.
-  have -> /= : to_uint (key{2} + W64.of_int 24) = to_uint key{2} + 24.  
-  + by rewrite W64.to_uintD_small //= /#.
-  have -> /= : to_uint (key{2} + W64.of_int 28) = to_uint key{2} + 28.  
-  + by rewrite W64.to_uintD_small //= /#.
-  have -> /= : to_uint (nonce{2} + W64.of_int 4) = to_uint nonce{2} + 4.
-  + by rewrite W64.to_uintD_small //= /#.
-  have -> /= : to_uint (nonce{2} + W64.of_int 8) = to_uint nonce{2} + 8.  
-  + by rewrite W64.to_uintD_small //= /#.
-  congr;apply W8u32.Pack.all_eq_eq => /=.
-  rewrite /W8u32.Pack.all_eq /= !W8u32.bits32_div //.
-  by rewrite /(%/) /=; do !rewrite -W32.of_int_mod /(%%) /=.
-qed.
-  
-equiv eq_increment_counter_x8 : ChaCha20_pavx2.M.increment_counter_x8 ~ M.increment_counter_x8 : 
-  s{2} = (x8 st1 st2 st3 st4 st5 st6 st7 st8){1} 
-  ==> 
-  res{2} = x8 res{1}.`1 res{1}.`2 res{1}.`3 res{1}.`4 res{1}.`5 res{1}.`6 res{1}.`7 res{1}.`8.
-proof.
-  proc => /=; wp; skip => /> &1.
-  rewrite -set_x8 1:// get_x8 1://; congr.
-  rewrite /x86_VPADD_8u32 /= /unpack32 /map2 /=; congr; apply W8u32.Pack.all_eq_eq => /=.
-  rewrite /W8u32.Pack.all_eq /= !W8u32.bits32_div //.
-  rewrite 8!(W32.WRingA.addrC _ (W32.of_int 8)).
-  by rewrite /(%/) /=; do !rewrite -W32.of_int_mod /(%%) /=.
-qed.
-
-op upd_mem (fs:(int -> W8.t) list) (mem:global_mem_t) (output:address) (j:int) = 
-  if in_range output (64 * size fs) j then
-    let j = j - output in 
-     (nth witness fs (j%/64)) (j%%64)
-  else mem.[j].
-
-lemma upd_mem_rcons f fs mem output j :
-  upd_mem (rcons fs f) mem output j = 
-  if in_range (output + 64 * size fs) 64 j then f ((j-output)%%64) 
-  else upd_mem fs mem output j.
-proof.
-  rewrite /upd_mem size_rcons.
-  case: (in_range (output + 64 * size fs) 64 j) => hj. 
-  + have -> /= : in_range output (64 * (size fs + 1)) j by smt(size_ge0).  
-    rewrite nth_rcons.
-    have -> : (j - output) %/ 64 = size fs.
-    have -> : j - output = (j-(output + 64 * size fs)) + size fs * 64 by ring.
-    + by rewrite divzMDr 1:// divz_small 2:// /#. 
-    by rewrite StdOrder.IntOrder.ltrr.
-  have -> : in_range output (64 * (size fs + 1)) j = in_range output (64 * size fs) j by smt(size_ge0). 
-  case: (in_range output (64 * size fs) j) => // hj1.
-  by rewrite /= nth_rcons ltz_divLR 1:// /#.
-qed.
-
-lemma upd_mem_one f mem output j :
-  upd_mem [f] mem output j = 
-  if in_range output 64 j then f ((j-output)%%64) 
-  else mem.[j].
-proof. rewrite (upd_mem_rcons f [] mem output j) /= /upd_mem /= /#. qed.
-
-op xor_mem (mem:global_mem_t) plain i (k:W32.t Array16.t) j = 
-  (WArray64.init32 (fun (i0 : int) => k.[i0])).[j] `^` mem.[plain + 64 * i + j].
-
-op mapi (n:int) (f:int -> 'a -> 'b) (xs:'a list) =
-  with xs = "[]" => []
-  with xs = (::) y ys => f n y :: mapi (n+1) f ys.
-
-lemma mapi_rcons n (f:int -> 'a -> 'b) xs x :
-   mapi n f (rcons xs x) = rcons (mapi n f xs) (f (n + size xs) x).
-proof. elim: xs n => //= xs hrec n;rewrite hrec /#. qed.
-
-lemma size_mapi  n (f:int -> 'a -> 'b) xs : size (mapi n f xs) = size xs.
-proof. by elim: xs n => //= xs hrec n;rewrite hrec. qed.
-
-hoare store64_spec output0 plain0 len0 k0 mem0 : ChaCha20_pref.M.store : 
-  output = output0 /\ plain = plain0 /\ len = len0 /\ k = k0 /\ Glob.mem = mem0 /\ 
-  64 <= len /\ inv_ptr output plain len 
-  ==>
-  inv_ptr res.`1 res.`2 res.`3 /\ 
-  res = (output0 + 64, plain0 + 64, len0 - 64) /\
-  forall j, 
-    Glob.mem.[j] = 
-      if in_range output0 64 j then
-        let j = j - output0 in
-        (WArray64.init32 (fun (i0 : int) => k0.[i0])).[j] `^` mem0.[plain0 + j]
-      else mem0.[j].
-proof.
-  proc; inline *; wp.
-  while (0 <= i <= min 64 len /\ 
-    forall j, Glob.mem.[j] = if in_range output i j then k8.[j - output] else mem0.[j]).
-  + wp; skip => /> &hr h0i _ hj hi; split; 1: smt().
-    by move=> j; rewrite storeW8E get_setE hj; smt().
-  wp; while(0 <= i <= min 64 len /\
-    forall j, 0 <= j < i => k8.[j] = k8_0.[j] `^` loadW8 Glob.mem (plain + j)).
-  + wp; skip => />; smt (WArray64.get_setE).
-  by wp; skip => /> /#.
-qed.
-
-op xor_mem_half (o:int) (mem:global_mem_t) output plain i (k:W32.t Array8.t) j = 
-  if o <= j < o + 32 then
-     (WArray32.init32
-       (fun (i0 : int) => k.[i0])).[j-o] `^` mem.[plain + 64 * i + j]
-  else mem.[output + 64 * i + j].
-
-op disj_or_eq (output plain len: int) = 
-   plain = output \/ plain + len <= output \/ output + len <= plain.
-
-lemma get_storeW128E m p w j: 
-    (storeW128 m p w).[j] = if p <= j < p + 16 then w \bits8 j - p else m.[j].
-proof. rewrite storeW128E /= get_storesE /= /#. qed.
-
-lemma get_storeW256E m p w j: 
-    (storeW256 m p w).[j] = if p <= j < p + 32 then w \bits8 j - p else m.[j].
-proof. rewrite storeW256E /= get_storesE /= /#. qed.
-
-module StoreHalfInt = {
-  proc store_half_x8
-    (output:int, plain:int, len:int, k:W256.t Array8.t, o:int) : unit =
-  {
-    var aux, i : int;
-    
-    i <- 0;
-    while (i < 8) {
-      k.[i] <- k.[i] `^` (loadW256 Glob.mem (plain + o + (64 * i)));
-      i <- i + 1;
-    }
-    i <- 0;
-    while (i < 8) {
-      Glob.mem <- storeW256 Glob.mem (output + o + (64 * i)) k.[i];
-      i <- i + 1;
-    }
-  }
-}.
-
-op half_x8 (k1 k2 k3 k4 k5 k6 k7 k8 : W32.t Array8.t) =
-  Array8.of_list witness [
-    W8u32.pack8 [k1.[0]; k1.[1]; k1.[2]; k1.[3]; k1.[4]; k1.[5]; k1.[6]; k1.[7]];
-    W8u32.pack8 [k2.[0]; k2.[1]; k2.[2]; k2.[3]; k2.[4]; k2.[5]; k2.[6]; k2.[7]];
-    W8u32.pack8 [k3.[0]; k3.[1]; k3.[2]; k3.[3]; k3.[4]; k3.[5]; k3.[6]; k3.[7]];
-    W8u32.pack8 [k4.[0]; k4.[1]; k4.[2]; k4.[3]; k4.[4]; k4.[5]; k4.[6]; k4.[7]];
-    W8u32.pack8 [k5.[0]; k5.[1]; k5.[2]; k5.[3]; k5.[4]; k5.[5]; k5.[6]; k5.[7]];
-    W8u32.pack8 [k6.[0]; k6.[1]; k6.[2]; k6.[3]; k6.[4]; k6.[5]; k6.[6]; k6.[7]];
-    W8u32.pack8 [k7.[0]; k7.[1]; k7.[2]; k7.[3]; k7.[4]; k7.[5]; k7.[6]; k7.[7]];
-    W8u32.pack8 [k8.[0]; k8.[1]; k8.[2]; k8.[3]; k8.[4]; k8.[5]; k8.[6]; k8.[7]]].
-
-lemma mapi_map2 n (f : int -> 'a -> 'b) (s : 'a list) :
-  mapi n f s = map2 (fun i x => f i x) (range n (n + size s)) s.
-proof.
-elim: s n => //= [@/range //|x s ih] n.
-rewrite (@range_cat (n + 1)); 1,2:smt(size_ge0).
-rewrite rangeS addzCA addzA (@addzC 1) -(@cat1s x).
-by rewrite map2_cat //= -ih.
-qed.
-
-lemma pack4_init (k:int ->  W32.t) : 
-  pack4 [k 0; k 1; k 2; k 3] = 
-  pack4_t (W4u32.Pack.init k).
-proof. by congr; apply W4u32.Pack.all_eq_eq; cbv delta. qed.
-
-lemma pack8_init (k:int -> W32.t) : 
-  pack8 [k 0; k 1; k 2; k 3; k 4; k 5; k 6; k 7] = 
-  pack8_t (W8u32.Pack.init k).
-proof. by congr; apply W8u32.Pack.all_eq_eq; cbv delta. qed.
-
-lemma get8_pack8u32 f j: 
-  pack8_t (W8u32.Pack.init f) \bits8 j = 
-    if 0 <= j < 32 then f (j %/ 4) \bits8 (j %% 4) else W8.zero.
-proof.
-  rewrite pack8E W8.wordP => i hi.
-  rewrite bits8E /= initE hi /= initE.
-  have -> /= : (0 <= j * 8 + i < 256) <=> (0 <= j < 32) by smt().
-  case : (0 <= j < 32) => hj //=.
-  rewrite bits8E /= initE.
-  have -> : (j * 8 + i) %/ 32 = j %/4.
-  + rewrite {1}(divz_eq j 4) mulzDl mulzA /= -addzA divzMDl //.
-    by rewrite (divz_small _ 32) //; smt (modz_cmp).
-  rewrite initE hi /= divz_cmp //=; congr.
-  rewrite {1}(divz_eq j 4) mulzDl mulzA /= -addzA modzMDl modz_small //; smt (modz_cmp).
-qed.
-
-hoare pavx2_half_store_x8_spec mem0 k1 k2 k3 k4 k5 k6 k7 k8 output0 plain0 len0 o0:
-  StoreHalfInt.store_half_x8 :
-       disj_or_eq output plain len
-    /\ k = half_x8 k1 k2 k3 k4 k5 k6 k7 k8
-    /\ (o0 = 0 \/ o0 = 32)
-    /\ output = output0
-    /\ plain = plain0
-    /\ o = o0
-    /\ len = len0
-    /\ 512 <= len
-    /\ Glob.mem = mem0 
-  ==>
-    forall j, Glob.mem.[j] =
-       upd_mem
-         (mapi 0 (xor_mem_half o0 mem0 output0 plain0)
-         [k1; k2; k3; k4; k5; k6; k7; k8]) mem0 output0 j.
-proof.
-  proc=> /=.
-  seq 2 : (#{~k=_}pre /\ forall j, 0 <= j < 8 => 
-    k.[j] = (half_x8 k1 k2 k3 k4 k5 k6 k7 k8).[j] `^` loadW256 mem0 (plain0 + o0 + 64 * j)).
-  sp; while {1} (0 <= i <= 8 /\ #[/2:]{~k=_}pre /\ forall j, 0 <= j < 8 =>
-    if j < i then
-      k.[j] = (half_x8 k1 k2 k3 k4 k5 k6 k7 k8).[j] `^` loadW256 Glob.mem (plain0 + o0 + 64 * j)
-    else k.[j] = (half_x8 k1 k2 k3 k4 k5 k6 k7 k8).[j]).
-  - by auto=> /> *; smt(Array8.get_setE).
-  - by auto=> /> /#.
-  pose T j := take j [k1; k2; k3; k4; k5; k6; k7; k8].
-  sp; while {1} (0 <= i <= 8 /\ #[/2:]{~Glob.mem=_}pre /\ forall (j : address),
-    Glob.mem.[j] = upd_mem
-      (mapi 0 (xor_mem_half o0 mem0 output0 plain0) (T i)) mem0 output0 j).
-  - auto=> /> &hr *; split; 1: by smt().
-    move=> j; rewrite /T (@take_nth witness) // -/(T _).
-    pose k' := nth _ _ _; rewrite mapi_rcons upd_mem_rcons.
-    rewrite size_mapi {1}/T size_take //= H6 /=.
-    rewrite get_storeW256E H5.
-    case (output{hr} + o{hr} + 64 * i{hr} <= j < output{hr} + o{hr} + 64 * i{hr} + 32) => hj.
-    + have -> /= : in_range (output{hr} + 64 * i{hr}) 64 j by smt().
-      rewrite /xor_mem_half. 
-      have -> : (j - output{hr}) %% 64 =  j - (output{hr} + 64 * i{hr}).
-      + have -> : j - output{hr} = j - (output{hr} + 64 * i{hr}) + i{hr} * 64 by ring.
-        by rewrite modzMDr modz_small /#.  
-      have -> /= : o{hr} <= j - (output{hr} + 64 * i{hr}) < o{hr} + 32 by smt().
-      rewrite H4 1:// W32u8.xorb8E; congr.
-      + rewrite /init32 initiE 1:/#. beta.
-        have -> : (half_x8 k1 k2 k3 k4 k5 k6 k7 k8).[i{hr}] = W8u32.pack8 (Array8.to_list k').
-        + rewrite /k'; have : i{hr} \in (iota_ 0 8) by rewrite mem_iota.
-          by move: (i{hr}); apply List.allP; rewrite /= /half_x8 /=.
-        rewrite /to_list /mkseq /= (pack8_init (fun j => k'.[j])) get8_pack8u32.
-        by have -> /# : 0 <= j - (output{hr} + o{hr} + 64 * i{hr}) < 32 by smt().
-      by rewrite /loadW256 pack32bE 1:/#  initiE 1:/# /= /#.
-    case (in_range (output{hr} + 64 * i{hr}) 64 j) => [hj1 | //].
-    rewrite {2}/xor_mem_half.
-    have -> : (j - output{hr}) %% 64 =  j - (output{hr} + 64 * i{hr}).
-    + have -> : j - output{hr} = j - (output{hr} + 64 * i{hr}) + i{hr} * 64 by ring.
-      by rewrite modzMDr modz_small /#.  
-    have -> : !(o{hr} <= j - (output{hr} + 64 * i{hr}) < o{hr} + 32) by smt().
-    rewrite /= /upd_mem size_mapi {1}/T size_take // /= H6 /= /#.
-  skip => /> /#.
-qed.
-
-hoare savx2_half_store_x8_spec mem0 k1 k2 k3 k4 k5 k6 k7 k8 output0 plain0 len0 o0:
-  M.store_half_x8 :
-       disj_or_eq output0 plain0 len0 /\ good_ptr output0 plain0 len0 
-    /\ k = half_x8 k1 k2 k3 k4 k5 k6 k7 k8
-    /\ (o0 = 0 \/ o0 = 32)
-    /\ to_uint output = output0
-    /\ to_uint plain = plain0
-    /\ o = o0
-    /\ to_uint len = len0
-    /\ 512 <= len0
-    /\ Glob.mem = mem0 
-  ==>
-    forall j, Glob.mem.[j] =
-       upd_mem
-         (mapi 0 (xor_mem_half o0 mem0 output0 plain0)
-         [k1; k2; k3; k4; k5; k6; k7; k8]) mem0 output0 j.
-proof.
-  bypr => &m [#] h1 h2 h3 h4 hout hplain ho hlen h5 hmem.
-  have <- : 
-    Pr[StoreHalfInt.store_half_x8(output0, plain0, len0, k{m}, o0) @ &m :
-      ! (forall (j : address),
-        Glob.mem.[j] =
-        upd_mem (mapi 0 (xor_mem_half o0 mem0 output0 plain0) [k1; k2; k3; k4; k5; k6; k7; k8]) mem0 output0 j)] =
-    Pr[M.store_half_x8(output{m}, plain{m}, len{m}, k{m}, o{m}) @ &m :
-      ! (forall (j : address),
-        Glob.mem.[j] =
-        upd_mem (mapi 0 (xor_mem_half o0 mem0 output0 plain0) [k1; k2; k3; k4; k5; k6; k7; k8]) mem0 output0 j)].
-  + byequiv (_ : output{1} = to_uint output{2} /\ plain{1} = to_uint plain{2} /\ len{1} = to_uint len{2} /\ 512 <= len{1} /\
-                 (o = 0 \/ o = 32){1} /\
-                 ={Glob.mem, o, k} /\ good_ptr output{1} plain{1} len{1} ==> ={Glob.mem}).
-    + proc.
-      while (={i,o,k,Glob.mem} /\ good_ptr output{1} plain{1} len{1} /\ 0 <= i{1} /\
-             output{1} = to_uint output{2} /\ 512 <= len{1} /\ (o = 0 \/ o = 32){1}).
-      + wp;skip => /> *;split;2:smt().
-        have h : to_uint (W64.of_int (o{2} + 64 * i{2})) = o{2} + 64 * i{2}.
-        + by apply W64.to_uint_small => /= /#.
-        by rewrite W64.to_uintD_small h /= /#.
-      wp; while (={i,o,k,Glob.mem} /\ good_ptr output{1} plain{1} len{1} /\ 0 <= i{1} /\
-             plain{1} = to_uint plain{2} /\ 512 <= len{1} /\ (o = 0 \/ o = 32){1}). 
-      + wp; skip=> /> *; split; 2:smt().
-        have h : to_uint (W64.of_int (o{2} + 64 * i{2})) = o{2} + 64 * i{2}.
-        + by apply W64.to_uint_small => /= /#.
-        by rewrite W64.to_uintD_small h /= /#.
-      by wp; skip => />.
-    + by move=> />; rewrite hout hplain hlen ho.
-    done.
-  byphoare (_:    disj_or_eq output plain len
-               /\ k = half_x8 k1 k2 k3 k4 k5 k6 k7 k8
-               /\ (o0 = 0 \/ o0 = 32)
-               /\ output = output0
-               /\ plain = plain0
-               /\ o = o0
-               /\ len = len0
-               /\ 512 <= len
-               /\ Glob.mem = mem0 
-             ==>
-               !forall j, Glob.mem.[j] =
-                  upd_mem
-                  (mapi 0 (xor_mem_half o0 mem0 output0 plain0)
-                  [k1; k2; k3; k4; k5; k6; k7; k8]) mem0 output0 j) => //.
-  by hoare; conseq (pavx2_half_store_x8_spec mem0 k1 k2 k3 k4 k5 k6 k7 k8 output0 plain0 len0 o0).
-qed.
-
-op x4 (k1 k2 k3 k4 k5 k6 k7 k8: W32.t Array8.t) =
-  Array8.init (fun i => W8u32.pack8 [k1.[i]; k2.[i]; k3.[i]; k4.[i]; k5.[i]; k6.[i]; k7.[i]; k8.[i]]).
-
-lemma W8u32_bits128_0 (w:W8u32.Pack.pack_t) :
-  pack8_t w \bits128 0 = pack4 [w.[0]; w.[1]; w.[2]; w.[3]].
-proof. by rewrite -{1}(W8u32.Pack.to_listK w) /= -pack2_4u32_8u32. qed.
-
-lemma W8u32_bits128_1 (w:W8u32.Pack.pack_t) :
-  pack8_t w \bits128 1 = pack4 [w.[4]; w.[5]; w.[6]; w.[7]].
-proof. by rewrite -{1}(W8u32.Pack.to_listK w) /= -pack2_4u32_8u32. qed.
-
-lemma pack2_2u32_4u32 (w0 w1 w2 w3 :W32.t) :
-   pack2 [pack2 [w0;w1]; pack2 [w2; w3]] =
-   pack4 [w0; w1; w2; w3].
-proof. by apply W128.all_eq_eq;cbv W128.all_eq (%/) (%%). qed.
-
-lemma W4u32_bits64_0 (w:W4u32.Pack.pack_t) :
-  pack4_t w \bits64 0 = pack2 [w.[0]; w.[1]].
-proof. by rewrite -{1}(W4u32.Pack.to_listK w) /= -pack2_2u32_4u32. qed.
-
-lemma W4u32_bits64_1 (w:W4u32.Pack.pack_t) :
-  pack4_t w \bits64 1 = pack2 [w.[2]; w.[3]].
-proof. by rewrite -{1}(W4u32.Pack.to_listK w) /= -pack2_2u32_4u32. qed.
-
-(*lemma W2u128_W8u32 (w:W2u128.Pack.pack_t) : 
-   pack2_t w = pack8 [w.[0] \bits32 0 ; w.[0] \bits32 1; w.[0] \bits32 2 ; w.[0] \bits32 3;
-                      w.[1] \bits32 0 ; w.[1] \bits32 1; w.[1] \bits32 2 ; w.[1] \bits32 3].
-proof.
-  rewrite -pack2_4u32_8u32; congr.
-  apply W2u128.Pack.all_eq_eq; rewrite /all_eq /=.
-  rewrite -{1}(W4u32.unpack32K w.[0]) -{1}(W4u32.unpack32K w.[1]).
-  by rewrite /unpack32;split;congr;rewrite W4u32.Pack.init_of_list.
-qed.*)
-
-hint simplify (W8u32_bits128_0, W8u32_bits128_1, W4u32_bits64_0, W4u32_bits64_1).
-
-lemma x86_VPUNPCKH_8u32_spec (v0 v1 v2 v3 v4 v5 v6 v7 : W32.t) 
-                             (w0 w1 w2 w3 w4 w5 w6 w7 : W32.t): 
-  x86_VPUNPCKH_8u32 (W8u32.pack8 [v0; v1; v2; v3; v4; v5; v6; v7])
-                    (W8u32.pack8 [w0; w1; w2; w3; w4; w5; w6; w7]) =
-  W8u32.pack8 [v2; w2; v3; w3; v6; w6; v7; w7].
-proof.
-  by cbv delta; rewrite -(pack2_4u32_8u32 v2); congr; apply W2u128.Pack.all_eq_eq; rewrite /all_eq.
-qed.
-
-lemma x86_VPUNPCKL_8u32_spec (v0 v1 v2 v3 v4 v5 v6 v7 : W32.t) 
-                             (w0 w1 w2 w3 w4 w5 w6 w7 : W32.t): 
-  x86_VPUNPCKL_8u32 (W8u32.pack8 [v0; v1; v2; v3; v4; v5; v6; v7])
-                    (W8u32.pack8 [w0; w1; w2; w3; w4; w5; w6; w7]) =
-  W8u32.pack8 [v0; w0; v1; w1; v4; w4; v5; w5].
-proof.
-  by cbv delta; rewrite -(pack2_4u32_8u32 v0 w0); congr; apply W2u128.Pack.all_eq_eq; rewrite /all_eq.
-qed.
-
-lemma x86_VPERM2I128_8u32_spec_32 (v0 v1 v2 v3 v4 v5 v6 v7 : W32.t) (w0 w1 w2 w3 w4 w5 w6 w7 : W32.t):
-  x86_VPERM2I128 (W8u32.pack8 [v0; v1; v2; v3; v4; v5; v6; v7]) (W8u32.pack8 [w0; w1; w2; w3; w4; w5; w6; w7]) (W8.of_int 32) =
-  W8u32.pack8 [v0; v1; v2; v3; w0; w1; w2; w3].
-proof.
-  by cbv delta; rewrite !of_intwE; cbv delta; rewrite pack2_4u32_8u32.
-qed.
-
-lemma x86_VPERM2I128_8u32_spec_49 (v0 v1 v2 v3 v4 v5 v6 v7 : W32.t) (w0 w1 w2 w3 w4 w5 w6 w7 : W32.t):
-  x86_VPERM2I128 (W8u32.pack8 [v0; v1; v2; v3; v4; v5; v6; v7]) (W8u32.pack8 [w0; w1; w2; w3; w4; w5; w6; w7]) (W8.of_int 49) =
-  W8u32.pack8 [v4; v5; v6; v7; w4; w5; w6; w7].
-proof.
-  by cbv delta; rewrite !of_intwE; cbv delta; rewrite pack2_4u32_8u32.
-qed.
-
-lemma x86_VPUNPCKL_4u64_8u32 (v0 v1 v2 v3 v4 v5 v6 v7 : W32.t) (w0 w1 w2 w3 w4 w5 w6 w7 : W32.t):
-  x86_VPUNPCKL_4u64 (W8u32.pack8 [v0; v1; v2; v3; v4; v5; v6; v7]) (W8u32.pack8 [w0; w1; w2; w3; w4; w5; w6; w7]) =
-  W8u32.pack8 [v0;v1;w0;w1;v4;v5;w4;w5].
-proof.
-  by cbv delta; rewrite W2u128.Pack.init_of_list /= !pack2_2u32_4u32 pack2_4u32_8u32 .
-qed.
-
-lemma x86_VPUNPCKH_4u64_8u32 (v0 v1 v2 v3 v4 v5 v6 v7 : W32.t) (w0 w1 w2 w3 w4 w5 w6 w7 : W32.t):
-  x86_VPUNPCKH_4u64 (W8u32.pack8 [v0; v1; v2; v3; v4; v5; v6; v7]) (W8u32.pack8 [w0; w1; w2; w3; w4; w5; w6; w7]) =
-  W8u32.pack8 [v2;v3;w2;w3;v6;v7;w6;w7].
-proof.
-  by cbv delta; rewrite W2u128.Pack.init_of_list /= !pack2_2u32_4u32 pack2_4u32_8u32 .
-qed.
-
-hint simplify (x86_VPUNPCKH_8u32_spec, x86_VPUNPCKL_8u32_spec, x86_VPERM2I128_8u32_spec_32, x86_VPERM2I128_8u32_spec_49,
-               x86_VPUNPCKL_4u64_8u32, x86_VPUNPCKH_4u64_8u32).
-
-hoare rotate_spec k1 k2 k3 k4 k5 k6 k7 k8 : ChaCha20_savx2.M.rotate :
-   x = x4 k1 k2 k3 k4 k5 k6 k7 k8 ==>
-   res = half_x8 k1 k2 k3 k4 k5 k6 k7 k8.
-proof.
-  conseq (_: Array8.all_eq res (half_x8 k1 k2 k3 k4 k5 k6 k7 k8)).
-  + by move=> *;apply Array8.all_eq_eq.
-  proc.
-  inline M.sub_rotate.
-  unroll for ^while.   
-  unroll for ^while.
-  wp; skip => &hr /= ->.
-  have -> : W8.of_int (1 %% 16 + 48) = W8.of_int 49 by cbv delta.
-  have -> : W8.of_int (0 %% 16 + 32) = W8.of_int 32 by cbv delta.
-  by rewrite /all_eq /x4 /half_x8 /= .
-qed.
-
-hoare rotate_stack_spec k1 k2 k3 k4 k5 k6 k7 k8 : ChaCha20_savx2.M.rotate_stack :
-   s = x4 k1 k2 k3 k4 k5 k6 k7 k8 ==>
-   res = half_x8 k1 k2 k3 k4 k5 k6 k7 k8.
-proof.
-  conseq (_: Array8.all_eq res (half_x8 k1 k2 k3 k4 k5 k6 k7 k8)).
-  + by move=> *;apply Array8.all_eq_eq.
-  proc.
-  inline M.sub_rotate.
-  do 3!(unroll for ^while).   
-  wp; skip => &hr /= ->.
-  have -> : W8.of_int (1 %% 16 + 48) = W8.of_int 49 by cbv delta.
-  have -> : W8.of_int (0 %% 16 + 32) = W8.of_int 32 by cbv delta.
-  by rewrite /all_eq /x4 /half_x8 /= .
-qed.
-
-op sub8 i (k:'a Array16.t) = Array8.of_list witness (Array16.sub k i 8).
-
-hoare rotate_first_half_x8_spec k1 k2 k3 k4 k5 k6 k7 k8 : M.rotate_first_half_x8 : 
-   k = x8 k1 k2 k3 k4 k5 k6 k7 k8 ==>
-   res.`1 = half_x8 (sub8 0 k1) (sub8 0 k2) (sub8 0 k3) (sub8 0 k4) (sub8 0 k5) (sub8 0 k6) (sub8 0 k7) (sub8 0 k8) /\
-   res.`2 = x4 (sub8 8 k1) (sub8 8 k2) (sub8 8 k3) (sub8 8 k4) (sub8 8 k5) (sub8 8 k6) (sub8 8 k7) (sub8 8 k8).
-proof.
-  proc.
-  ecall (rotate_spec (sub8 0 k1) (sub8 0 k2) (sub8 0 k3) (sub8 0 k4) (sub8 0 k5) (sub8 0 k6) (sub8 0 k7) (sub8 0 k8)).
-  while (0 <= i <= 8 /\ forall j, 0 <= j < i => k0_7.[j] = k.[j]).
-  + by wp; skip; smt (Array8.get_setE).
-  wp; while (0 <= i <= 8 /\ forall j, 0 <= j < i => s_k8_15.[j] = k.[8 + j]).
-  + by wp; skip; smt (Array8.get_setE).
-  wp; skip => />; split; 1:smt().
-  move=> i0 s_k8_15 ??? h1; split; 1:smt().
-  move=> i1 k0_7 ??? h2.
-  have ->> : i0 = 8 by smt().
-  have ->> : i1 = 8 by smt().
-  split; apply Array8.all_eq_eq; rewrite /Array8.all_eq /=.
-  + by rewrite !h2; cbv delta.
-  by rewrite !h1; cbv delta.
-qed.
-
-lemma sub8_second_half k j: 
-  32 <= j < 64 =>
-  (WArray32.init32 ("_.[_]" (sub8 8 k))).[j - 32] = (WArray64.init32 ("_.[_]" k)).[j].
-proof.
-  move=> h;rewrite /WArray32.init32 /WArray64.init32 !initiE /=.
-  + smt (). + smt().
-  rewrite /sub8 /= /Array16.sub /mkseq /=.
-  have -> : -32 = (-8) * 4 by done.
-  rewrite modzMDr divzMDr 1://;congr.
-  have hj1 : 8 <= j %/ 4 < 16.
-  + rewrite lez_divRL //= ltz_divLR //.
-  by rewrite  Array8.get_of_list /#.
-qed.
-
-lemma sub8_first_half k j: 
-  0 <= j < 32 =>
-  (WArray32.init32 ("_.[_]" (sub8 0 k))).[j] = (WArray64.init32 ("_.[_]" k)).[j].
-proof.
-  move=> h;rewrite /WArray32.init32 /WArray64.init32 !initiE /=.
-  + smt (). + smt().
-  rewrite /sub8 /= /Array16.sub /mkseq /=.
-  have hj1 : 0 <= j %/ 4 < 8.
-  + rewrite lez_divRL //= ltz_divLR //.
-  by rewrite  Array8.get_of_list /#.
-qed.
-
-lemma nth_mapi k (f: int -> 'a -> 'b) al dfl j : 
-  nth dfl (mapi k f al) j = 
-   if 0 <= j < size al then f (k+j) (nth witness al j) else dfl.
-proof. elim: al k j => /= [ /# | a al hrec k j]; smt(size_ge0). qed.
-
-lemma upd_mem_mapi_8 output (f : int -> W32.t Array8.t -> int -> W8.t) ks mem j: 
-   upd_mem (mapi 0 f ks) mem output j = 
-    if in_range output (64 * size ks) j then
-      f ((j - output) %/64) (nth witness ks ((j - output) %/64)) ((j-output) %% 64)
-    else mem.[j].
-proof. 
-  rewrite /upd_mem size_mapi; case: (in_range output (64 * size ks) j) => //= hin.
-  rewrite nth_mapi ltz_divLR 1:// lez_divRL 1:// /= /#.
-qed.
-
-lemma upd_mem_mapi_16 output (f : int -> W32.t Array16.t -> int -> W8.t) ks mem j: 
-   upd_mem (mapi 0 f ks) mem output j = 
-    if in_range output (64 * size ks) j then
-      f ((j - output) %/64) (nth witness ks ((j - output) %/64)) ((j-output) %% 64)
-    else mem.[j].
-proof. 
-  rewrite /upd_mem size_mapi; case: (in_range output (64 * size ks) j) => //= hin.
-  rewrite nth_mapi ltz_divLR 1:// lez_divRL 1:// /= /#.
-qed.
-
-lemma upd_mem_half_2 len (mem1 mem0 mem2:global_mem_t) output plain k1 k2 k3 k4 k5 k6 k7 k8:
-  disj_or_eq output plain len =>  512 <= len => 
-  (forall (j : address),
-      mem1.[j] =
-      upd_mem (mapi 0 (xor_mem_half 0 mem0 output plain)
-                 [sub8 0 k1; sub8 0 k2; sub8 0 k3; sub8 0 k4; sub8 0 k5; sub8 0 k6; sub8 0 k7; sub8 0 k8]) mem0 output j) =>
-  (forall (j : address),
-      mem2.[j] =
-      upd_mem (mapi 0 (xor_mem_half 32 mem1 output plain)
-                 [sub8 8 k1; sub8 8 k2; sub8 8 k3; sub8 8 k4; sub8 8 k5; sub8 8 k6; sub8 8 k7; sub8 8 k8]) mem1 output j) =>
-   (forall (j:address),
-      mem2.[j] = 
-         upd_mem (mapi 0 (xor_mem mem0 plain) [k1; k2; k3; k4; k5; k6; k7; k8]) mem0 output j).
-proof.
-  move=> hd hlen hmem1 hmem2 j.
-  rewrite upd_mem_mapi_16 hmem2 upd_mem_mapi_8.
-  have -> : [sub8 8 k1; sub8 8 k2; sub8 8 k3; sub8 8 k4; sub8 8 k5; sub8 8 k6; sub8 8 k7; sub8 8 k8] = 
-            map (sub8 8) [k1;k2;k3;k4;k5;k6;k7;k8] by done.
-  have heq : [sub8 0 k1; sub8 0 k2; sub8 0 k3; sub8 0 k4; sub8 0 k5; sub8 0 k6; sub8 0 k7; sub8 0 k8] = 
-            map (sub8 0) [k1;k2;k3;k4;k5;k6;k7;k8] by done.
-  have hs : size [k1; k2; k3; k4; k5; k6; k7; k8] = 8 by done.
-  rewrite size_map hs.
-  pose k := nth witness [k1; k2; k3; k4; k5; k6; k7; k8] ((j - output) %/ 64).
-  case _ : (in_range output (64 * 8) j) => /= hj;last first.
-  + by rewrite hmem1 /upd_mem size_mapi /= hj.
-  rewrite (nth_map witness witness (sub8 8) ((j - output) %/ 64) [k1;k2;k3;k4;k5;k6;k7;k8]).
-  + by rewrite lez_divRL 1:// ltz_divLR //= /#.
-  rewrite -/k /xor_mem_half /xor_mem.
-  case: (32 <= (j -output) %% 64 < 32 + 32) => h. 
-  + congr; 1: by apply sub8_second_half.
-    rewrite hmem1 upd_mem_mapi_8 heq size_map hs.
-    pose k' := (map (sub8 0) [k1; k2; k3; k4; k5; k6; k7; k8]).   
-    case: (in_range output (64 * 8) (plain + 64 * ((j - output) %/ 64) + (j - output) %% 64)) => [h1 | //].
-    have ->> : plain = output by smt(divz_eq).
-    have -> : output + 64 * ((j - output) %/ 64) + (j - output) %% 64 - output = 
-              (j - output) %% 64 + ((j - output) %/ 64) * 64 by ring.
-    rewrite modzMDr divzMDr 1:// modz_mod (divz_small ((j - output) %% 64)); 1:smt(modz_cmp).
-    rewrite /= /k' (nth_map witness witness (sub8 0)).
-    + by rewrite lez_divRL 1:// ltz_divLR //= /#.
-    rewrite -/k /xor_mem_half; smt(modz_cmp).
-  rewrite hmem1 upd_mem_mapi_8 heq size_map hs.
-  pose k' := (map (sub8 0) [k1; k2; k3; k4; k5; k6; k7; k8]). 
-  have -> /= : output + 64 * ((j - output) %/ 64) + (j - output) %% 64 = j by smt(divz_eq).  
-  rewrite hj /= /k' (nth_map witness witness (sub8 0)).
-  + by rewrite lez_divRL 1:// ltz_divLR //= /#.
-  rewrite -/k /xor_mem_half. 
-  have h1 :  0 <= (j - output) %% 64 < 0 + 32 by smt(modz_cmp).
-  by rewrite h1 /=; congr; rewrite sub8_first_half.
-qed.
-
-hoare savx2_store_x8_spec mem0 k1 k2 k3 k4 k5 k6 k7 k8 output0 plain0 len0:
-  ChaCha20_savx2.M.store_x8 : 
-    disj_or_eq output0 plain0 len0 /\ good_ptr output0 plain0 len0 /\
-    k = x8 k1 k2 k3 k4 k5 k6 k7 k8 /\ 
-    to_uint output = output0 /\ to_uint plain = plain0 /\ to_uint len = len0 /\ 512 <= len0 /\ Glob.mem = mem0 
-    ==>
-    to_uint res.`1 = output0 + 512 /\ to_uint res.`2 = plain0 + 512 /\ to_uint res.`3 = len0 - 512 /\
-    (forall j, 
-       Glob.mem.[j] =
-       upd_mem (mapi 0 (xor_mem mem0 plain0) [k1; k2; k3; k4; k5; k6; k7; k8]) mem0 output0 j).
-proof.
-  proc.
-  inline M.update_ptr;wp.
-  ecall (savx2_half_store_x8_spec Glob.mem{hr} (sub8 8 k1) (sub8 8 k2) (sub8 8 k3) (sub8 8 k4) (sub8 8 k5) (sub8 8 k6) (sub8 8 k7) (sub8 8 k8)
-            output0 plain0 len0 32).
-  inline M.rotate_second_half_x8;wp.
-  ecall (rotate_stack_spec (sub8 8 k1) (sub8 8 k2) (sub8 8 k3) (sub8 8 k4) (sub8 8 k5) (sub8 8 k6) (sub8 8 k7) (sub8 8 k8)).
-  wp.
-  ecall (savx2_half_store_x8_spec Glob.mem{hr} (sub8 0 k1) (sub8 0 k2) (sub8 0 k3) (sub8 0 k4) (sub8 0 k5) (sub8 0 k6) (sub8 0 k7) (sub8 0 k8)
-            output0 plain0 len0 0).
-  ecall (rotate_first_half_x8_spec k1 k2 k3 k4 k5 k6 k7 k8); wp; skip => /> &hr h1 h2 h3 h4 [r1 r2] /= ?? mem1 w1 mem2 w2.
-  rewrite !W64.to_uintD_small /= 1..2:/#.
-  rewrite W32.to_uintB 1:uleE 1:// /=.
-  by apply (upd_mem_half_2 (to_uint len{hr}) mem1 Glob.mem{hr} mem2 (to_uint output{hr}) (to_uint plain{hr}) k1 k2 k3 k4 k5 k6 k7 k8).
-qed.
-
-phoare store_half_x8_ll : [ M.store_half_x8 : true ==> true] = 1%r.
-proof.
-  proc.
-  while true (8 - i); 1: by move=> z;auto => /#.
-  wp; while true (8 - i); 1: by move=> z;auto => /#.
-  by auto => /#.
-qed.
-
-phoare sub_rotate_ll : [ M.sub_rotate : true ==> true] = 1%r.   
-proof. by proc; while true (4 - i); auto => /#. qed.
-
-phoare savx2_store_x8 mem0 k1 k2 k3 k4 k5 k6 k7 k8 output0 plain0 len0:
-  [ChaCha20_savx2.M.store_x8 : 
-    disj_or_eq output0 plain0 len0 /\ good_ptr output0 plain0 len0 /\
-    k = x8 k1 k2 k3 k4 k5 k6 k7 k8 /\ 
-    to_uint output = output0 /\ to_uint plain = plain0 /\ to_uint len = len0 /\ 512 <= len0 /\ Glob.mem = mem0 
-    ==>
-    to_uint res.`1 = output0 + 512 /\ to_uint res.`2 = plain0 + 512 /\ to_uint res.`3 = len0 - 512 /\
-    (forall j, 
-       Glob.mem.[j] =
-       upd_mem (mapi 0 (xor_mem mem0 plain0) [k1; k2; k3; k4; k5; k6; k7; k8]) mem0 output0 j)] = 1%r.
-proof.
-  conseq (_: true ==> true) (savx2_store_x8_spec mem0 k1 k2 k3 k4 k5 k6 k7 k8 output0 plain0 len0);1:done.
-  proc;  inline M.rotate_second_half_x8 M.rotate_first_half_x8 M.rotate M.rotate_stack.
-  call (_: true); 1: by auto.
-  call store_half_x8_ll; wp.
-  call sub_rotate_ll; wp.
-  while true (4 - i1); 1: by auto => /#.
-  wp; while true (4 - i1); 1: by auto => /#.
-  wp; call store_half_x8_ll; wp.
-  call sub_rotate_ll; wp.
-  wp; while true (4 - i0); 1: by auto => /#.
-  wp; while true (8 - i); 1: by auto => /#.
-  wp; while true (8 - i); auto => /#.
-qed.
-
-lemma upd_mem_comp (mem0 mem1 mem2:global_mem_t) output plain len ks (k:W32.t Array16.t) : 
-   inv_ptr output plain len =>
-   64 * size ks + 64 <= len =>
-   let ofs = 64 * size ks in
-   (forall j, mem1.[j] = upd_mem (mapi 0 (xor_mem mem0 plain) ks) mem0 output j) =>
-   (forall j, mem2.[j] = 
-         if in_range (output + ofs) 64 j then
-            (WArray64.init32 (fun (i0 : int) => k.[i0])).[j - (output + ofs)] `^`
-             mem1.[plain + ofs + (j - (output + ofs))]
-         else mem1.[j]) =>
-   forall j, mem2.[j] = upd_mem (mapi 0 (xor_mem mem0 plain) (rcons ks k)) mem0 output j.
-proof.
-  move=> /= hinv hlen hmem1 hupd j.
-  rewrite mapi_rcons upd_mem_rcons hupd size_mapi !hmem1.
-  case: (in_range (output + 64 * size ks) 64 j) => [hj | //].
-  rewrite /upd_mem /= size_mapi /xor_mem.
-  have -> /= : !in_range output (64 * size ks) (plain + 64 * size ks + (j - (output + 64 * size ks))) by smt (size_ge0).
-  have -> // : j - (output + 64*size ks) = (j - output) %% 64.
-  have -> : j - output = j - (output + 64*size ks) + size ks * 64 by ring.
-  by rewrite modzMDr modz_small /#.  
-qed.
-  
-phoare pref_store_ll : [ChaCha20_pref.M.store : true ==> true] = 1%r.
-proof.
-  proc;inline *;wp.
-  while true (min 64 len -i).
-  + by move=> z; wp; skip => /#.
-  wp; while true (min 64 len -i).
-  + by move=> z; wp; skip => /#.
-  by wp; skip => /#.  
-qed.
-
-phoare pavx2_store_x8_spec mem0 k1 k2 k3 k4 k5 k6 k7 k8 output0 plain0 len0:
-  [ ChaCha20_pavx2_cf.M.store_x8 : 
-    inv_ptr output plain len /\
-    k_1 = k1 /\ k_2 = k2 /\ k_3 = k3 /\ k_4 = k4 /\ k_5 = k5 /\ k_6 = k6 /\ k_7 = k7 /\ k_8 = k8 /\
-    output = output0 /\ plain = plain0 /\ len = len0 /\ 512 <= len /\ Glob.mem = mem0 
-    ==>
-    res = (output0 + 512, plain0 + 512, len0 - 512) /\
-    (forall j, 
-       Glob.mem.[j] =
-       upd_mem (mapi 0 (xor_mem mem0 plain0) [k1; k2; k3; k4; k5; k6; k7; k8]) mem0 output0 j)] = 1%r.
-proof.
-  conseq  (_: true ==> true) (_: 
-    inv_ptr output plain len /\
-    k_1 = k1 /\ k_2 = k2 /\ k_3 = k3 /\ k_4 = k4 /\ k_5 = k5 /\ k_6 = k6 /\ k_7 = k7 /\ k_8 = k8 /\
-    output = output0 /\ plain = plain0 /\ len = len0 /\ 512 <= len /\ Glob.mem = mem0 
-    ==>
-    res = (output0 + 512, plain0 + 512, len0 - 512) /\
-    (forall j, 
-       Glob.mem.[j] =
-       upd_mem (mapi 0 (xor_mem mem0 plain0) [k1; k2; k3; k4; k5; k6; k7; k8]) mem0 output0 j)); last first.
-  + by proc; do 8!call pref_store_ll; skip.
-  + by move=> />.
-  proc => /=.
-  ecall (store64_spec output{hr} plain{hr} len{hr} k8 Glob.mem{hr}).
-  ecall (store64_spec output{hr} plain{hr} len{hr} k7 Glob.mem{hr}).
-  ecall (store64_spec output{hr} plain{hr} len{hr} k6 Glob.mem{hr}).
-  ecall (store64_spec output{hr} plain{hr} len{hr} k5 Glob.mem{hr}).
-  ecall (store64_spec output{hr} plain{hr} len{hr} k4 Glob.mem{hr}).
-  ecall (store64_spec output{hr} plain{hr} len{hr} k3 Glob.mem{hr}).
-  ecall (store64_spec output{hr} plain{hr} len{hr} k2 Glob.mem{hr}).
-  ecall (store64_spec output{hr} plain{hr} len{hr} k1 Glob.mem{hr}).
-  skip. move=> &hr [#] hinv 11!->> ? ->> /= />.
-  split; [smt() | move=> h1 h2 {h1 h2} mem1 hinv1 hmem1].
-  split; [smt() | move=> h {h} mem2 hinv2 hmem2].
-  split; [smt() | move=> h {h} mem3 hinv3 hmem3].
-  split; [smt() | move=> h {h} mem4 hinv4 hmem4].
-  split; [smt() | move=> h {h} mem5 hinv5 hmem5].
-  split; [smt() | move=> h {h} mem6 hinv6 hmem6].
-  split; [smt() | move=> h {h} mem7 hinv7 hmem7].
-  split; [smt() | move=> h {h} mem8 hinv8 hmem8].
-  have hup1 := upd_mem_comp mem0 mem0 mem1 output0 plain0 len0 [] k1 hinv _ _ hmem1.
-  + smt(). + by move=> j /=; rewrite /upd_mem /= (_:!in_range output0 0 j) 1:/#.
-  have hup2 := upd_mem_comp mem0 mem1 mem2 output0 plain0 len0 [k1] k2 hinv _ hup1 hmem2; 1: by smt().
-  have hup3 := upd_mem_comp mem0 mem2 mem3 output0 plain0 len0 [k1;k2] k3 hinv _ hup2 hmem3; 1: by smt().
-  have hup4 := upd_mem_comp mem0 mem3 mem4 output0 plain0 len0 [k1;k2;k3] k4 hinv _ hup3 hmem4; 1: by smt().
-  have hup5 := upd_mem_comp mem0 mem4 mem5 output0 plain0 len0 [k1;k2;k3;k4] k5 hinv _ hup4 hmem5; 1: by smt().
-  have hup6 := upd_mem_comp mem0 mem5 mem6 output0 plain0 len0 [k1;k2;k3;k4;k5] k6 hinv _ hup5 hmem6; 1: by smt().
-  have hup7 := upd_mem_comp mem0 mem6 mem7 output0 plain0 len0 [k1;k2;k3;k4;k5;k6] k7 hinv _ hup6 hmem7; 1: by smt().
-  by apply (upd_mem_comp mem0 mem7 mem8 output0 plain0 len0 [k1;k2;k3;k4;k5;k6;k7] k8 hinv _ hup7 hmem8); smt().
-qed.
-
-equiv eq_store_x8 : ChaCha20_pavx2_cf.M.store_x8 ~  M.store_x8 :
-  k{2} = (x8 k_1 k_2 k_3 k_4 k_5 k_6 k_7 k_8){1} /\ 
-  output{1} = to_uint output{2} /\ plain{1} = to_uint plain{2} /\ len{1} = to_uint len{2} /\
-  (good_ptr output plain len){1} /\ disj_or_eq output{1} plain{1} len{1} /\ 512 <= len{1} /\
-  ={Glob.mem} 
-  ==>
-  res{1}.`1 = to_uint res{2}.`1 /\ res{1}.`2 = to_uint res{2}.`2 /\ res{1}.`3 = to_uint res{2}.`3 /\ 
-  (good_ptr res{1}.`1 res{1}.`2 res{1}.`3){1} /\ (disj_or_eq res{1}.`1 res{1}.`2 res{1}.`3){1} /\
-  ={Glob.mem}.
-proof.
-  proc *.
-  ecall{1} (pavx2_store_x8_spec Glob.mem{1} k_1{1} k_2{1} k_3{1} k_4{1} k_5{1} k_6{1} k_7{1} k_8{1} output{1} plain{1} len{1}).
-  ecall{2} (savx2_store_x8 Glob.mem{1} k_1{1} k_2{1} k_3{1} k_4{1} k_5{1} k_6{1} k_7{1} k_8{1} output{1} plain{1} len{1}).
-  skip => |> &1 &2 _ 3!-> hg hd hlen /= [r1 r2 r3] mem1 /= 3!-> hmem1; split; 1:smt().
-  move=> _ mem2 hmem2 /=;split; [smt() | split;1:smt()].
-  by apply Jasmin_memory.mem_eq_ext => j;rewrite hmem1 hmem2.
-qed.
-
-equiv eq_store_x8_last : ChaCha20_pavx2_cf.M.store_x8_last ~  M.store_x8_last :
-  k{2} = (x8 k_1 k_2 k_3 k_4 k_5 k_6 k_7 k_8){1} /\
-  output{1} = to_uint output{2} /\ plain{1} = to_uint plain{2} /\ len{1} = to_uint len{2} /\
-  (good_ptr output plain len){1} /\ disj_or_eq output{1} plain{1} len{1} /\ 
-  ={Glob.mem} 
-  ==>
-  ={Glob.mem}.
-proof.
-admitted.
-
-equiv eq_sum_states_x8 : ChaCha20_pavx2.M.sum_states_x8 ~ M.sum_states_x8 :
-  k{2} = (x8 k1 k2 k3 k4 k5 k6 k7 k8){1} /\
-  st{2} = (x8 st1 st2 st3 st4 st5 st6 st7 st8){1} 
-  ==>
-  res{2} = x8 res{1}.`1 res{1}.`2 res{1}.`3 res{1}.`4 res{1}.`5 res{1}.`6 res{1}.`7 res{1}.`8.
-proof.
-  proc => /=.
-  inline *.
-  transitivity*{1} { 
-    i <- 0;
-    while (i < 16) {
-      k1.[i] <- k1.[i] + st1.[i];
-      k2.[i] <- k2.[i] + st2.[i];
-      k3.[i] <- k3.[i] + st3.[i];
-      k4.[i] <- k4.[i] + st4.[i];
-      k5.[i] <- k5.[i] + st5.[i];
-      k6.[i] <- k6.[i] + st6.[i];
-      k7.[i] <- k7.[i] + st7.[i];
-      k8.[i] <- k8.[i] + st8.[i];
-      i <- i + 1;
-    }
-  }. + smt(). + done.
-  + by do 8! unroll for{1} ^while; unroll for{2} ^while; wp; skip => />.
-  while (={i} /\ #pre /\ 0 <= i{1}); 2: by auto.
-  wp; skip => /> &1 &2 ??; split; 2:smt().
-  by rewrite !get_x8 1,2:// -set_x8 1:// /x86_VPADD_8u32.
-qed.
-
-equiv eq_chacha20_more_than_256 : 
-  ChaCha20_pavx2.M.chacha20_more_than_256 ~ ChaCha20_savx2.M.chacha20_more_than_256 : 
-  output{1} = to_uint output{2} /\ plain{1} = to_uint plain{2} /\ len{1} = to_uint len{2} /\
-  key{1} = to_uint key{2} /\ nonce{1} = to_uint nonce{2} /\ ={counter,Glob.mem} /\
-  (key + 32 < W64.modulus /\ nonce + 12 < W64.modulus){1} /\
-  (good_ptr output plain len){1} /\ (disj_or_eq output plain len){1} 
-  ==>
-  ={Glob.mem}.
-proof.
-  proc => /=.
-  seq 1 4 : (s_r16{2} = g_r16 /\ s_r8{2} = g_r8 /\ st{2} = (x8 st1 st2 st3 st4 st5 st6 st7 st8){1} /\
-            output{1} = to_uint output{2} /\ plain{1} = to_uint plain{2} /\ len{1} = to_uint len{2} /\
-            (good_ptr output plain len){1} /\ (disj_or_eq output plain len){1} /\ ={Glob.mem}).
-  + call eq_init_x8; inline{2} M.load_shufb_cmd; wp; skip => />.
-  seq 1 1 : (#pre).
-  + while (#pre). 
-    + call eq_increment_counter_x8 => /=.
-      call eq_store_x8 => /=.
-      call eq_sum_states_x8 => /=.   
-      call eq_rounds_x8 => /=. 
-      by inline M.copy_state_x8; wp; skip => |> &2 hg hd hl _ [r11 ri2 r13] [r21 r22 r23] /= 3!->> _ _;rewrite uleE.
-    by skip => |> *; rewrite uleE.
-  if; last by done.
-  + by move=> /> *; rewrite ultE.
-  call eq_store_x8_last.
-  call eq_sum_states_x8 => /=.   
-  call eq_rounds_x8 => /=. 
-  inline M.copy_state_x8; wp; skip => />.
-qed.
-
 (* --------------------------------------------------------------------- *)
 (*  chach20_less_than_257                                                *)
 
@@ -1071,6 +77,11 @@ proof.
   by rewrite pack2K initiE //= get_unpack32 // loadW64_bits32.
 qed.
 
+lemma pack2_2u32_4u32 (w0 w1 w2 w3 :W32.t) :
+   pack2 [pack2 [w0;w1]; pack2 [w2; w3]] =
+   pack4 [w0; w1; w2; w3].
+proof. by apply W128.all_eq_eq;cbv W128.all_eq (%/) (%%). qed.
+
 equiv eq_init_x2 :
   ChaCha20_pavx2.M.init_x2 ~ ChaCha20_savx2.M.init_x2 : 
   key{1} = to_uint key{2} /\ nonce{1} = to_uint nonce{2} /\ ={counter,Glob.mem} /\
@@ -1108,6 +119,40 @@ qed.
 lemma pack8_init_shift8 (k:W32.t Array16.t) : 
   pack8 [k.[8]; k.[9]; k.[10]; k.[11]; k.[12]; k.[13]; k.[14]; k.[15]] = 
   pack8_t (W8u32.Pack.init (fun i => k.[8 + i])).
+proof. by congr; apply W8u32.Pack.all_eq_eq; cbv delta. qed.
+
+lemma get8_pack8u32 f j: 
+  pack8_t (W8u32.Pack.init f) \bits8 j = 
+    if 0 <= j < 32 then f (j %/ 4) \bits8 (j %% 4) else W8.zero.
+proof.
+  rewrite pack8E W8.wordP => i hi.
+  rewrite bits8E /= initE hi /= initE.
+  have -> /= : (0 <= j * 8 + i < 256) <=> (0 <= j < 32) by smt().
+  case : (0 <= j < 32) => hj //=.
+  rewrite bits8E /= initE.
+  have -> : (j * 8 + i) %/ 32 = j %/4.
+  + rewrite {1}(divz_eq j 4) mulzDl mulzA /= -addzA divzMDl //.
+    by rewrite (divz_small _ 32) //; smt (modz_cmp).
+  rewrite initE hi /= divz_cmp //=; congr.
+  rewrite {1}(divz_eq j 4) mulzDl mulzA /= -addzA modzMDl modz_small //; smt (modz_cmp).
+qed.
+
+lemma get_storeW128E m p w j: 
+    (storeW128 m p w).[j] = if p <= j < p + 16 then w \bits8 j - p else m.[j].
+proof. rewrite storeW128E /= get_storesE /= /#. qed.
+
+lemma get_storeW256E m p w j: 
+    (storeW256 m p w).[j] = if p <= j < p + 32 then w \bits8 j - p else m.[j].
+proof. rewrite storeW256E /= get_storesE /= /#. qed.
+
+lemma pack4_init (k:int ->  W32.t) : 
+  pack4 [k 0; k 1; k 2; k 3] = 
+  pack4_t (W4u32.Pack.init k).
+proof. by congr; apply W4u32.Pack.all_eq_eq; cbv delta. qed.
+
+lemma pack8_init (k:int -> W32.t) : 
+  pack8 [k 0; k 1; k 2; k 3; k 4; k 5; k 6; k 7] = 
+  pack8_t (W8u32.Pack.init k).
 proof. by congr; apply W8u32.Pack.all_eq_eq; cbv delta. qed.
 
 lemma store_256_xor_spec output (k1:W32.t Array16.t) mem plain j:
@@ -1680,6 +725,17 @@ proof.
   by apply W8u32.Pack.all_eq_eq; apply (hall i); apply mema_iota.
 qed.
 
+(* Move this *)
+lemma x86_8u32_rol_xor r w : 0 < r < 32 => 
+  x86_VPSLL_8u32 w (W8.of_int r) `^` x86_VPSRL_8u32 w (W8.of_int (32 - r))  =
+  map (transpose W32.rol r) w.
+proof.
+  move=> hr;rewrite /x86_VPSRL_8u32 /x86_VPSLL_8u32 /(`>>`) /(`<<`).
+  rewrite !W8.to_uint_small /= 1,2:/# /=.
+  rewrite /map; congr; apply W8u32.Pack.ext_eq => j hj.
+  by rewrite map2iE 1:// 3!initE hj /= W32.rol_xor 1:/# 2?modz_small 1,2:/#.
+qed.
+
 phoare rotate_x8 k0 i0 r0 : 
   [M.rotate_x8 : 
     k = k0 /\ i = i0 /\ r = r0 /\ 0 <= i < 4 /\ 0 < r < 32 /\ r16 = g_r16 /\ r8 = g_r8 
@@ -1828,6 +884,1210 @@ proof.
   call eq_sum_states_x2.
   call eq_rounds_x2.
   by inline M.copy_state_x2; auto => /> /#.
+qed.
+
+(* ***************************************************************************************************************)
+(* ChaCha20_more_than_256                                                                                        *)
+
+op x8 (k1 k2 k3 k4 k5 k6 k7 k8: W32.t Array16.t) =
+  Array16.init (fun i => W8u32.pack8 [k1.[i]; k2.[i]; k3.[i]; k4.[i]; k5.[i]; k6.[i]; k7.[i]; k8.[i]]).
+(*
+  Array16.of_list W256.zero [
+     W8u32.pack8 [k1.[0 ]; k2.[0 ]; k3.[0 ]; k4.[0 ]; k5.[0 ]; k6.[0 ]; k7.[0 ]; k8.[0 ]];
+     W8u32.pack8 [k1.[1 ]; k2.[1 ]; k3.[1 ]; k4.[1 ]; k5.[1 ]; k6.[1 ]; k7.[1 ]; k8.[1 ]];
+     W8u32.pack8 [k1.[2 ]; k2.[2 ]; k3.[2 ]; k4.[2 ]; k5.[2 ]; k6.[2 ]; k7.[2 ]; k8.[2 ]];
+     W8u32.pack8 [k1.[3 ]; k2.[3 ]; k3.[3 ]; k4.[3 ]; k5.[3 ]; k6.[3 ]; k7.[3 ]; k8.[3 ]];
+     W8u32.pack8 [k1.[4 ]; k2.[4 ]; k3.[4 ]; k4.[4 ]; k5.[4 ]; k6.[4 ]; k7.[4 ]; k8.[4 ]];
+     W8u32.pack8 [k1.[5 ]; k2.[5 ]; k3.[5 ]; k4.[5 ]; k5.[5 ]; k6.[5 ]; k7.[5 ]; k8.[5 ]];
+     W8u32.pack8 [k1.[6 ]; k2.[6 ]; k3.[6 ]; k4.[6 ]; k5.[6 ]; k6.[6 ]; k7.[6 ]; k8.[6 ]];
+     W8u32.pack8 [k1.[7 ]; k2.[7 ]; k3.[7 ]; k4.[7 ]; k5.[7 ]; k6.[7 ]; k7.[7 ]; k8.[7 ]];
+     W8u32.pack8 [k1.[8 ]; k2.[8 ]; k3.[8 ]; k4.[8 ]; k5.[8 ]; k6.[8 ]; k7.[8 ]; k8.[8 ]];
+     W8u32.pack8 [k1.[9 ]; k2.[9 ]; k3.[9 ]; k4.[9 ]; k5.[9 ]; k6.[9 ]; k7.[9 ]; k8.[9 ]];
+     W8u32.pack8 [k1.[10]; k2.[10]; k3.[10]; k4.[10]; k5.[10]; k6.[10]; k7.[10]; k8.[10]];
+     W8u32.pack8 [k1.[11]; k2.[11]; k3.[11]; k4.[11]; k5.[11]; k6.[11]; k7.[11]; k8.[11]];
+     W8u32.pack8 [k1.[12]; k2.[12]; k3.[12]; k4.[12]; k5.[12]; k6.[12]; k7.[12]; k8.[12]];
+     W8u32.pack8 [k1.[13]; k2.[13]; k3.[13]; k4.[13]; k5.[13]; k6.[13]; k7.[13]; k8.[13]];
+     W8u32.pack8 [k1.[14]; k2.[14]; k3.[14]; k4.[14]; k5.[14]; k6.[14]; k7.[14]; k8.[14]];
+     W8u32.pack8 [k1.[15]; k2.[15]; k3.[15]; k4.[15]; k5.[15]; k6.[15]; k7.[15]; k8.[15]]
+  ].
+*)
+
+lemma get_x8 (k1 k2 k3 k4 k5 k6 k7 k8: W32.t Array16.t) i: 
+  0 <= i < 16 => 
+  (x8 k1 k2 k3 k4 k5 k6 k7 k8).[i] = 
+     W8u32.pack8 [k1.[i]; k2.[i]; k3.[i]; k4.[i]; k5.[i]; k6.[i]; k7.[i]; k8.[i]].
+proof.
+  by move => h; rewrite /x8 initE h.
+qed.
+
+lemma set_x8 (k1 k2 k3 k4 k5 k6 k7 k8: W32.t Array16.t) i w1 w2 w3 w4 w5 w6 w7 w8: 
+  0 <= i < 16 =>
+  (x8 k1 k2 k3 k4 k5 k6 k7 k8).[i <- W8u32.pack8 [w1;w2;w3;w4;w5;w6;w7;w8]] =
+  x8 k1.[i<-w1] k2.[i<-w2] k3.[i<-w3] k4.[i<-w4] k5.[i<-w5] k6.[i<-w6] k7.[i<-w7] k8.[i<-w8].
+proof.
+  move=> hi; apply Array16.ext_eq => j hj.  
+  rewrite /x8 setE 2!initE hj /= initE hj /= !Array16.get_set_if hi /=.
+  by case: (j = i).
+qed.
+
+phoare rotate_x8_s k0 i0 r0 : 
+  [M.rotate_x8_s : 
+    k = k0 /\ i = i0 /\ r = r0 /\ 0 <= i < 16 /\ 0 < r < 32 /\ r16 = g_r16 /\ r8 = g_r8 
+    ==>
+    res = k0.[i0 <- W8u32.pack8_t (W8u32.Pack.map (fun (x:W32.t) => rol x r0) (W8u32.unpack32 k0.[i0]))]] = 1%r.
+proof.
+  proc => /=.
+  if; 1: by wp;skip.  
+  if; 1: by wp;skip.
+  wp;skip => /> &m hi1 hi2 hr1 hr2 _ _; congr.
+  by rewrite W256.xorwC get_setE 1:// /= x86_8u32_rol_xor.
+qed.
+
+equiv eq_line_x8_v_ a_ c_ k_ : ChaCha20_pavx2.M.line_x1_8 ~ M._line_x8_v :
+  ={a,b,c,r} /\ k{2} = k_ /\ a{1} = a_ /\ c{1} = c_ /\
+   k{2} = (x8 k1 k2 k3 k4 k5 k6 k7 k8){1} /\ 
+   0 <= a{1} < 16 /\ 0 <= b{1} < 16 /\ 0 <= c{1} < 16 /\ 0 < r{1} < 32 /\
+   r16{2} = g_r16 /\ r8{2} = g_r8 
+  ==> 
+  res{2} = x8 res{1}.`1 res{1}.`2 res{1}.`3 res{1}.`4 res{1}.`5 res{1}.`6 res{1}.`7 res{1}.`8 /\
+  forall i, 0 <= i < 16 => i <> a_ => i <> c_ => res{2}.[i] = k_.[i].
+proof.
+  proc => /=.
+  inline{1} ChaCha20_pref.M.line.
+  interleave{1} [2:4] [11:4] [20:4] [29:4] [38:4] [47:4] [56:4] [65:4] 1.
+  swap{1} 1 32.
+  interleave{1} [33:1] [38:1] [43:1] [48:1] [53:1] [58:1] [63:1] [68:1] 5.
+  sp 32 0.
+  seq 16 1 : (#{/~k{2}}pre /\ k{2} = (x8 k k0 k9 k10 k11 k12 k13 k14){1} /\
+                forall i, 0 <= i < 16 => i <> a_ => i <> c_ => k{2}.[i] = k_.[i]).
+  + wp;skip => /> &1 &2 ha1 ha2 hb1 hb2 hc1 hc2 hr1 hr2.
+    split; 1: by rewrite /x86_VPADD_8u32 !get_x8 1,2:// -set_x8.
+    by move=> ??? h ?;rewrite Array16.get_setE // h.
+  seq 8 1 : (#pre). 
+  + wp;skip => /> &1 &2 ha1 ha2 hb1 hb2 hc1 hc2 hr1 hr2 hi.
+    split; 1: by rewrite !get_x8 1,2:// -set_x8.
+    by move=> ???? h;rewrite Array16.get_setE // h /= hi.
+  wp;ecall{2} (rotate_x8_s k{2} c{2} r{2}); skip => /> &1 &2 ha1 ha2 hb1 hb2 hc1 hc2 hr1 hr2 hi.
+  split; 1: by rewrite !get_x8 1,2:// -set_x8.
+  by move=> ???? h;rewrite Array16.get_setE // h /= hi.
+qed.
+
+equiv eq_line_2 a0_ c0_ a1_ c1_ k_ :  ChaCha20_pavx2.M.line_2_x1_8 ~ M.line_x8_v : 
+  ={a0,b0,c0,r0,a1,b1,c1,r1} /\ k{2} = k_ /\ a0{1} = a0_ /\ c0{1} = c0_ /\ a1{1} = a1_ /\ c1{1} = c1_ /\
+   k{2} = (x8 k1 k2 k3 k4 k5 k6 k7 k8){1} /\ 
+   0 <= a0{1} < 16 /\ 0 <= b0{1} < 16 /\ 0 <= c0{1} < 16 /\ 0 < r0{1} < 32 /\
+   0 <= a1{1} < 16 /\ 0 <= b1{1} < 16 /\ 0 <= c1{1} < 16 /\ 0 < r1{1} < 32 /\
+   r16{2} = g_r16 /\ r8{2} = g_r8 
+  ==> 
+  res{2} = x8 res{1}.`1 res{1}.`2 res{1}.`3 res{1}.`4 res{1}.`5 res{1}.`6 res{1}.`7 res{1}.`8 /\
+  forall i, 0 <= i < 16 => i <> a0_ => i <> c0_ => i <> a1_ => i <> c1_ => res{2}.[i] = k_.[i].
+proof.
+  proc => /=.
+  inline{1} ChaCha20_pavx2.M.line_2.
+  interleave{1} [2:8] [18:8] [34:8] [50:8] [66:8] [82:8] [98:8] [114:8] 1.
+  swap{1} 1 64.
+  interleave{1} [65:1] [73:1] [81:1] [89:1] [97:1] [105:1] [113:1] [121:1] 8.
+  sp 64 0.
+  seq 16 1 : (#{/~k{2}}pre /\ k{2} = (x8 k k0 k9 k10 k11 k12 k13 k14){1} /\
+     forall i, 0 <= i < 16 => i <> a0_ => i <> c0_ => i <> a1_ => i <> c1_ => k{2}.[i] = k_.[i]).
+  + wp;skip => /> &1 &2 ha1 ha2 hb1 hb2 hc1 hc2 hd1 hd2 ha1' ha2' hb1' hb2' hc1' hc2' hd1' hd2'.
+    split; 1: by rewrite /x86_VPADD_8u32 !get_x8 1,2:// -set_x8.
+    by move=> ??? h *;rewrite Array16.get_setE // h.
+  seq 8 1 : (#pre).
+  + wp;skip => /> &1 &2 ha1 ha2 hb1 hb2 hc1 hc2 hd1 hd2 ha1' ha2' hb1' hb2' hc1' hc2' hd1' hd2' hi.
+    split; 1: by rewrite /x86_VPADD_8u32 !get_x8 1,2:// -set_x8. 
+    by move=> ????? h *;rewrite Array16.get_setE // h /= hi.
+  seq 8 1 : (#pre). 
+  + wp;skip => /> &1 &2 ha1 ha2 hb1 hb2 hc1 hc2 hd1 hd2 ha1' ha2' hb1' hb2' hc1' hc2' hd1' hd2' hi.
+    split; 1: by rewrite !get_x8 1,2:// -set_x8.
+    by move=> ???? h *;rewrite Array16.get_setE // h /= hi.
+  seq 8 1 : (#pre). 
+  + wp;skip => /> &1 &2 ha1 ha2 hb1 hb2 hc1 hc2 hd1 hd2 ha1' ha2' hb1' hb2' hc1' hc2' hd1' hd2' hi.
+    split; 1: by rewrite !get_x8 1,2:// -set_x8.
+    by move=> ?????? h;rewrite Array16.get_setE // h /= hi.
+  seq 8 1 : (#pre).
+  + wp; ecall{2} (rotate_x8_s k{2} c0{2} r0{2}); skip => /> 
+      &1 &2 ha1 ha2 hb1 hb2 hc1 hc2 hd1 hd2 ha1' ha2' hb1' hb2' hc1' hc2' hd1' hd2' hi.
+    split; 1: by rewrite !get_x8 1,2:// -set_x8.
+    by move=> ???? h *;rewrite Array16.get_setE // h /= hi.
+  wp; ecall{2} (rotate_x8_s k{2} c1{2} r1{2}); skip => /> 
+    &1 &2 ha1 ha2 hb1 hb2 hc1 hc2 hd1 hd2 ha1' ha2' hb1' hb2' hc1' hc2' hd1' hd2' hi.
+  split; 1: by rewrite !get_x8 1,2:// -set_x8.
+  by move=> ?????? h;rewrite Array16.get_setE // h /= hi.
+qed.
+
+equiv eq_double_quarter_round_x8 a0_ b0_ c0_ d0_ a1_ b1_ c1_ d1_ k_ : 
+    ChaCha20_pavx2.M.double_quarter_round_x8 ~ 
+    ChaCha20_savx2.M.double_quarter_round_x8: 
+    ={a0,b0,c0,d0,a1,b1,c1,d1} /\
+     k{2} = k_ /\ a0{1} = a0_ /\ b0{1} = b0_ /\ c0{1} = c0_ /\ d0{1} = d0_ /\
+                  a1{1} = a1_ /\ b1{1} = b1_ /\ c1{1} = c1_ /\ d1{1} = d1_ /\ 
+     k{2} = (x8 k1 k2 k3 k4 k5 k6 k7 k8){1}  /\ 
+     0 <= a0{1} < 16 /\ 0 <= b0{1} < 16 /\ 0 <= c0{1} < 16 /\ 0 <= d0{1} < 16  /\
+     0 <= a1{1} < 16 /\ 0 <= b1{1} < 16 /\ 0 <= c1{1} < 16 /\ 0 <= d1{1} < 16  /\
+     r16{2} = g_r16 /\ r8{2} = g_r8 
+    ==> 
+    res{2} = x8 res{1}.`1 res{1}.`2 res{1}.`3 res{1}.`4 res{1}.`5 res{1}.`6 res{1}.`7 res{1}.`8 /\
+     forall i, 0 <= i < 16 => i <> a0_ => i <> b0_ => i <> c0_ => i <> d0_ =>
+                             i <> a1_ => i <> b1_ => i <> c1_ => i <> d1_ =>
+               res{2}.[i] = k_.[i].
+proof.
+  proc => /=; wp.
+  ecall (eq_line_x8_v_ c1_ b1_ k{2})=> /=.
+  ecall (eq_line_2 c0_ b0_ a1_ d1_ k{2})=> /=.
+  ecall (eq_line_2 a0_ d0_ c1_ b1_ k{2})=> /=.
+  ecall (eq_line_2 c0_ b0_ a1_ d1_ k{2})=> /=.
+  ecall (eq_line_x8_v_ a0_ d0_ k{2})=> /=; skip => /> /#.
+qed.
+
+equiv eq_column_round_x8 : ChaCha20_pavx2.M.column_round_x8 ~ ChaCha20_savx2.M.column_round_x8 : 
+  k{2} = (x8 k1 k2 k3 k4 k5 k6 k7 k8){1}  /\
+   k15{2} = k{2}.[15] /\ s_r16{2} = g_r16 /\ s_r8{2} = g_r8 
+  ==> 
+  res{2}.`1 = x8 res{1}.`1 res{1}.`2 res{1}.`3 res{1}.`4 res{1}.`5 res{1}.`6 res{1}.`7 res{1}.`8 /\
+   res{2}.`2 = res{2}.`1.[14].
+proof.
+  proc => /=; wp.
+  ecall (eq_double_quarter_round_x8 1 5 9 13 3 7 11 15 k{2}); wp => /=.
+  ecall (eq_double_quarter_round_x8 0 4 8 12 2 6 10 14 k{2}); wp => /=.
+  skip => /> &1 r1 hi.
+  by rewrite -(hi 15) // Array16.set_notmod /= => r2 ->. 
+qed.
+
+equiv eq_diagonal_round_x8 : ChaCha20_pavx2.M.diagonal_round_x8 ~ ChaCha20_savx2.M.diagonal_round_x8 : 
+  k{2} = (x8 k1 k2 k3 k4 k5 k6 k7 k8){1}  /\
+   k14{2} = k{2}.[14] /\ s_r16{2} = g_r16 /\ s_r8{2} = g_r8 
+  ==> 
+  res{2}.`1 = x8 res{1}.`1 res{1}.`2 res{1}.`3 res{1}.`4 res{1}.`5 res{1}.`6 res{1}.`7 res{1}.`8 /\
+   res{2}.`2 = res{2}.`1.[15].
+proof.
+  proc => /=; wp.
+  ecall (eq_double_quarter_round_x8 2 7 8 13 3 4 9 14 k{2}); wp => /=.
+  ecall (eq_double_quarter_round_x8 1 6 11 12 0 5 10 15 k{2}); wp => /=.
+  skip => /> &1 r1 hi.
+  by rewrite -(hi 14) // Array16.set_notmod /= => r2 ->. 
+qed.
+
+equiv eq_rounds_x8 : ChaCha20_pavx2.M.rounds_x8 ~ ChaCha20_savx2.M.rounds_x8 :
+  k{2} = (x8 k1 k2 k3 k4 k5 k6 k7 k8){1} /\ s_r16{2} = g_r16 /\ s_r8{2} = g_r8 
+  ==> 
+  res{2} = x8 res{1}.`1 res{1}.`2 res{1}.`3 res{1}.`4 res{1}.`5 res{1}.`6 res{1}.`7 res{1}.`8.
+proof.
+  proc => /=; wp.
+  while (#pre /\ c{1} = W64.to_uint c{2} /\ (k15 = k.[15]){2}).
+  + wp; call eq_diagonal_round_x8; call eq_column_round_x8; skip => /> *.
+    rewrite ultE /=;rewrite to_uintD_small //= 1:/#.
+  by wp; skip => /> *;rewrite Array16.set_notmod.
+qed.
+ 
+equiv eq_init_x8 : ChaCha20_pavx2.M.init_x8 ~ M.init_x8 : 
+  key{1} = to_uint key{2} /\ nonce{1} = to_uint nonce{2} /\ ={counter,Glob.mem} /\
+  (key + 32 < W64.modulus /\ nonce + 12 < W64.modulus){1} 
+  ==>
+  res{2} = x8 res{1}.`1 res{1}.`2 res{1}.`3 res{1}.`4 res{1}.`5 res{1}.`6 res{1}.`7 res{1}.`8.
+proof.
+  proc => /=.
+  inline ChaCha20_pref.M.init.
+  do 2! unroll for{1} ^while; do 2! unroll for{2} ^while.
+  conseq (_ : Array16.all_eq st_{2} (x8 st1{1} st2{1} st3{1} st4{1} st5{1} st6{1} st7{1} st8{1})).
+  + by move=> *; apply Array16.all_eq_eq.
+  wp; skip; cbv delta => /> &2 h1 h2.
+  have -> /= : to_uint (key{2} + W64.of_int 4) = to_uint key{2} + 4.
+  + by rewrite W64.to_uintD_small //= /#.
+  have -> /= : to_uint (key{2} + W64.of_int 8) = to_uint key{2} + 8.  
+  + by rewrite W64.to_uintD_small //= /#.
+  have -> /= : to_uint (key{2} + W64.of_int 12) = to_uint key{2} + 12.  
+  + by rewrite W64.to_uintD_small //= /#.
+  have -> /= : to_uint (key{2} + W64.of_int 16) = to_uint key{2} + 16.  
+  + by rewrite W64.to_uintD_small //= /#.
+  have -> /= : to_uint (key{2} + W64.of_int 20) = to_uint key{2} + 20.  
+  + by rewrite W64.to_uintD_small //= /#.
+  have -> /= : to_uint (key{2} + W64.of_int 24) = to_uint key{2} + 24.  
+  + by rewrite W64.to_uintD_small //= /#.
+  have -> /= : to_uint (key{2} + W64.of_int 28) = to_uint key{2} + 28.  
+  + by rewrite W64.to_uintD_small //= /#.
+  have -> /= : to_uint (nonce{2} + W64.of_int 4) = to_uint nonce{2} + 4.
+  + by rewrite W64.to_uintD_small //= /#.
+  have -> /= : to_uint (nonce{2} + W64.of_int 8) = to_uint nonce{2} + 8.  
+  + by rewrite W64.to_uintD_small //= /#.
+  congr;apply W8u32.Pack.all_eq_eq => /=.
+  rewrite /W8u32.Pack.all_eq /= !W8u32.bits32_div //.
+  by rewrite /(%/) /=; do !rewrite -W32.of_int_mod /(%%) /=.
+qed.
+  
+equiv eq_increment_counter_x8 : ChaCha20_pavx2.M.increment_counter_x8 ~ M.increment_counter_x8 : 
+  s{2} = (x8 st1 st2 st3 st4 st5 st6 st7 st8){1} 
+  ==> 
+  res{2} = x8 res{1}.`1 res{1}.`2 res{1}.`3 res{1}.`4 res{1}.`5 res{1}.`6 res{1}.`7 res{1}.`8.
+proof.
+  proc => /=; wp; skip => /> &1.
+  rewrite -set_x8 1:// get_x8 1://; congr.
+  rewrite /x86_VPADD_8u32 /= /unpack32 /map2 /=; congr; apply W8u32.Pack.all_eq_eq => /=.
+  rewrite /W8u32.Pack.all_eq /= !W8u32.bits32_div //.
+  rewrite 8!(W32.WRingA.addrC _ (W32.of_int 8)).
+  by rewrite /(%/) /=; do !rewrite -W32.of_int_mod /(%%) /=.
+qed.
+
+op upd_mem (fs:(int -> W8.t) list) (mem:global_mem_t) (output:address) (j:int) = 
+  if in_range output (64 * size fs) j then
+    let j = j - output in 
+     (nth witness fs (j%/64)) (j%%64)
+  else mem.[j].
+
+lemma upd_mem_rcons f fs mem output j :
+  upd_mem (rcons fs f) mem output j = 
+  if in_range (output + 64 * size fs) 64 j then f ((j-output)%%64) 
+  else upd_mem fs mem output j.
+proof.
+  rewrite /upd_mem size_rcons.
+  case: (in_range (output + 64 * size fs) 64 j) => hj. 
+  + have -> /= : in_range output (64 * (size fs + 1)) j by smt(size_ge0).  
+    rewrite nth_rcons.
+    have -> : (j - output) %/ 64 = size fs.
+    have -> : j - output = (j-(output + 64 * size fs)) + size fs * 64 by ring.
+    + by rewrite divzMDr 1:// divz_small 2:// /#. 
+    by rewrite StdOrder.IntOrder.ltrr.
+  have -> : in_range output (64 * (size fs + 1)) j = in_range output (64 * size fs) j by smt(size_ge0). 
+  case: (in_range output (64 * size fs) j) => // hj1.
+  by rewrite /= nth_rcons ltz_divLR 1:// /#.
+qed.
+
+lemma upd_mem_one f mem output j :
+  upd_mem [f] mem output j = 
+  if in_range output 64 j then f ((j-output)%%64) 
+  else mem.[j].
+proof. rewrite (upd_mem_rcons f [] mem output j) /= /upd_mem /= /#. qed.
+
+op xor_mem (mem:global_mem_t) plain i (k:W32.t Array16.t) j = 
+  (WArray64.init32 (fun (i0 : int) => k.[i0])).[j] `^` mem.[plain + 64 * i + j].
+
+op mapi (n:int) (f:int -> 'a -> 'b) (xs:'a list) =
+  with xs = "[]" => []
+  with xs = (::) y ys => f n y :: mapi (n+1) f ys.
+
+lemma mapi_rcons n (f:int -> 'a -> 'b) xs x :
+   mapi n f (rcons xs x) = rcons (mapi n f xs) (f (n + size xs) x).
+proof. elim: xs n => //= xs hrec n;rewrite hrec /#. qed.
+
+lemma size_mapi  n (f:int -> 'a -> 'b) xs : size (mapi n f xs) = size xs.
+proof. by elim: xs n => //= xs hrec n;rewrite hrec. qed.
+
+hoare store64_spec output0 plain0 len0 k0 mem0 : ChaCha20_pref.M.store : 
+  output = output0 /\ plain = plain0 /\ len = len0 /\ k = k0 /\ Glob.mem = mem0 /\ 
+  64 <= len /\ inv_ptr output plain len 
+  ==>
+  inv_ptr res.`1 res.`2 res.`3 /\ 
+  res = (output0 + 64, plain0 + 64, len0 - 64) /\
+  forall j, 
+    Glob.mem.[j] = 
+      if in_range output0 64 j then
+        let j = j - output0 in
+        (WArray64.init32 (fun (i0 : int) => k0.[i0])).[j] `^` mem0.[plain0 + j]
+      else mem0.[j].
+proof.
+  proc; inline *; wp.
+  while (0 <= i <= min 64 len /\ 
+    forall j, Glob.mem.[j] = if in_range output i j then k8.[j - output] else mem0.[j]).
+  + wp; skip => /> &hr h0i _ hj hi; split; 1: smt().
+    by move=> j; rewrite storeW8E get_setE hj; smt().
+  wp; while(0 <= i <= min 64 len /\
+    forall j, 0 <= j < i => k8.[j] = k8_0.[j] `^` loadW8 Glob.mem (plain + j)).
+  + wp; skip => />; smt (WArray64.get_setE).
+  by wp; skip => /> /#.
+qed.
+
+op xor_mem_half (o:int) (mem:global_mem_t) output plain i (k:W32.t Array8.t) j = 
+  if o <= j < o + 32 then
+     (WArray32.init32
+       (fun (i0 : int) => k.[i0])).[j-o] `^` mem.[plain + 64 * i + j]
+  else mem.[output + 64 * i + j].
+
+op disj_or_eq (output plain len: int) = 
+   plain = output \/ plain + len <= output \/ output + len <= plain.
+
+module StoreHalfInt = {
+  proc store_half_x8
+    (output:int, plain:int, len:int, k:W256.t Array8.t, o:int) : unit =
+  {
+    var aux, i : int;
+    
+    i <- 0;
+    while (i < 8) {
+      k.[i] <- k.[i] `^` (loadW256 Glob.mem (plain + o + (64 * i)));
+      i <- i + 1;
+    }
+    i <- 0;
+    while (i < 8) {
+      Glob.mem <- storeW256 Glob.mem (output + o + (64 * i)) k.[i];
+      i <- i + 1;
+    }
+  }
+}.
+
+op half_x8 (k1 k2 k3 k4 k5 k6 k7 k8: W32.t Array8.t) =
+  Array8.init (fun i => W8u32.pack8 [k1.[i]; k2.[i]; k3.[i]; k4.[i]; k5.[i]; k6.[i]; k7.[i]; k8.[i]]).
+
+op half_x8_ (k1 k2 k3 k4 k5 k6 k7 k8 : W32.t Array8.t) =
+  Array8.of_list witness [
+    W8u32.pack8 [k1.[0]; k1.[1]; k1.[2]; k1.[3]; k1.[4]; k1.[5]; k1.[6]; k1.[7]];
+    W8u32.pack8 [k2.[0]; k2.[1]; k2.[2]; k2.[3]; k2.[4]; k2.[5]; k2.[6]; k2.[7]];
+    W8u32.pack8 [k3.[0]; k3.[1]; k3.[2]; k3.[3]; k3.[4]; k3.[5]; k3.[6]; k3.[7]];
+    W8u32.pack8 [k4.[0]; k4.[1]; k4.[2]; k4.[3]; k4.[4]; k4.[5]; k4.[6]; k4.[7]];
+    W8u32.pack8 [k5.[0]; k5.[1]; k5.[2]; k5.[3]; k5.[4]; k5.[5]; k5.[6]; k5.[7]];
+    W8u32.pack8 [k6.[0]; k6.[1]; k6.[2]; k6.[3]; k6.[4]; k6.[5]; k6.[6]; k6.[7]];
+    W8u32.pack8 [k7.[0]; k7.[1]; k7.[2]; k7.[3]; k7.[4]; k7.[5]; k7.[6]; k7.[7]];
+    W8u32.pack8 [k8.[0]; k8.[1]; k8.[2]; k8.[3]; k8.[4]; k8.[5]; k8.[6]; k8.[7]]].
+
+lemma mapi_map2 n (f : int -> 'a -> 'b) (s : 'a list) :
+  mapi n f s = map2 (fun i x => f i x) (range n (n + size s)) s.
+proof.
+elim: s n => //= [@/range //|x s ih] n.
+rewrite (@range_cat (n + 1)); 1,2:smt(size_ge0).
+rewrite rangeS addzCA addzA (@addzC 1) -(@cat1s x).
+by rewrite map2_cat //= -ih.
+qed.
+
+hoare pavx2_half_store_x8_spec mem0 k1 k2 k3 k4 k5 k6 k7 k8 output0 plain0 len0 o0:
+  StoreHalfInt.store_half_x8 :
+       disj_or_eq output plain len
+    /\ k = half_x8_ k1 k2 k3 k4 k5 k6 k7 k8
+    /\ (o0 = 0 \/ o0 = 32)
+    /\ output = output0
+    /\ plain = plain0
+    /\ o = o0
+    /\ len = len0
+    /\ 512 <= len
+    /\ Glob.mem = mem0 
+  ==>
+    forall j, Glob.mem.[j] =
+       upd_mem
+         (mapi 0 (xor_mem_half o0 mem0 output0 plain0)
+         [k1; k2; k3; k4; k5; k6; k7; k8]) mem0 output0 j.
+proof.
+  proc=> /=.
+  seq 2 : (#{~k=_}pre /\ forall j, 0 <= j < 8 => 
+    k.[j] = (half_x8_ k1 k2 k3 k4 k5 k6 k7 k8).[j] `^` loadW256 mem0 (plain0 + o0 + 64 * j)).
+  sp; while {1} (0 <= i <= 8 /\ #[/2:]{~k=_}pre /\ forall j, 0 <= j < 8 =>
+    if j < i then
+      k.[j] = (half_x8_ k1 k2 k3 k4 k5 k6 k7 k8).[j] `^` loadW256 Glob.mem (plain0 + o0 + 64 * j)
+    else k.[j] = (half_x8_ k1 k2 k3 k4 k5 k6 k7 k8).[j]).
+  - by auto=> /> *; smt(Array8.get_setE).
+  - by auto=> /> /#.
+  pose T j := take j [k1; k2; k3; k4; k5; k6; k7; k8].
+  sp; while {1} (0 <= i <= 8 /\ #[/2:]{~Glob.mem=_}pre /\ forall (j : address),
+    Glob.mem.[j] = upd_mem
+      (mapi 0 (xor_mem_half o0 mem0 output0 plain0) (T i)) mem0 output0 j).
+  - auto=> /> &hr *; split; 1: by smt().
+    move=> j; rewrite /T (@take_nth witness) // -/(T _).
+    pose k' := nth _ _ _; rewrite mapi_rcons upd_mem_rcons.
+    rewrite size_mapi {1}/T size_take //= H6 /=.
+    rewrite get_storeW256E H5.
+    case (output{hr} + o{hr} + 64 * i{hr} <= j < output{hr} + o{hr} + 64 * i{hr} + 32) => hj.
+    + have -> /= : in_range (output{hr} + 64 * i{hr}) 64 j by smt().
+      rewrite /xor_mem_half. 
+      have -> : (j - output{hr}) %% 64 =  j - (output{hr} + 64 * i{hr}).
+      + have -> : j - output{hr} = j - (output{hr} + 64 * i{hr}) + i{hr} * 64 by ring.
+        by rewrite modzMDr modz_small /#.  
+      have -> /= : o{hr} <= j - (output{hr} + 64 * i{hr}) < o{hr} + 32 by smt().
+      rewrite H4 1:// W32u8.xorb8E; congr.
+      + rewrite /init32 initiE 1:/#. beta.
+        have -> : (half_x8_ k1 k2 k3 k4 k5 k6 k7 k8).[i{hr}] = W8u32.pack8 (Array8.to_list k').
+        + rewrite /k'; have : i{hr} \in (iota_ 0 8) by rewrite mem_iota.
+          by move: (i{hr}); apply List.allP; rewrite /= /half_x8_ /=.
+        rewrite /to_list /mkseq /= (pack8_init (fun j => k'.[j])) get8_pack8u32.
+        by have -> /# : 0 <= j - (output{hr} + o{hr} + 64 * i{hr}) < 32 by smt().
+      by rewrite /loadW256 pack32bE 1:/#  initiE 1:/# /= /#.
+    case (in_range (output{hr} + 64 * i{hr}) 64 j) => [hj1 | //].
+    rewrite {2}/xor_mem_half.
+    have -> : (j - output{hr}) %% 64 =  j - (output{hr} + 64 * i{hr}).
+    + have -> : j - output{hr} = j - (output{hr} + 64 * i{hr}) + i{hr} * 64 by ring.
+      by rewrite modzMDr modz_small /#.  
+    have -> : !(o{hr} <= j - (output{hr} + 64 * i{hr}) < o{hr} + 32) by smt().
+    rewrite /= /upd_mem size_mapi {1}/T size_take // /= H6 /= /#.
+  skip => /> /#.
+qed.
+
+hoare savx2_half_store_x8_spec mem0 k1 k2 k3 k4 k5 k6 k7 k8 output0 plain0 len0 o0:
+  M.store_half_x8 :
+       disj_or_eq output0 plain0 len0 /\ good_ptr output0 plain0 len0 
+    /\ k = half_x8_ k1 k2 k3 k4 k5 k6 k7 k8
+    /\ (o0 = 0 \/ o0 = 32)
+    /\ to_uint output = output0
+    /\ to_uint plain = plain0
+    /\ o = o0
+    /\ to_uint len = len0
+    /\ 512 <= len0
+    /\ Glob.mem = mem0 
+  ==>
+    forall j, Glob.mem.[j] =
+       upd_mem
+         (mapi 0 (xor_mem_half o0 mem0 output0 plain0)
+         [k1; k2; k3; k4; k5; k6; k7; k8]) mem0 output0 j.
+proof.
+  bypr => &m [#] h1 h2 h3 h4 hout hplain ho hlen h5 hmem.
+  have <- : 
+    Pr[StoreHalfInt.store_half_x8(output0, plain0, len0, k{m}, o0) @ &m :
+      ! (forall (j : address),
+        Glob.mem.[j] =
+        upd_mem (mapi 0 (xor_mem_half o0 mem0 output0 plain0) [k1; k2; k3; k4; k5; k6; k7; k8]) mem0 output0 j)] =
+    Pr[M.store_half_x8(output{m}, plain{m}, len{m}, k{m}, o{m}) @ &m :
+      ! (forall (j : address),
+        Glob.mem.[j] =
+        upd_mem (mapi 0 (xor_mem_half o0 mem0 output0 plain0) [k1; k2; k3; k4; k5; k6; k7; k8]) mem0 output0 j)].
+  + byequiv (_ : output{1} = to_uint output{2} /\ plain{1} = to_uint plain{2} /\ len{1} = to_uint len{2} /\ 512 <= len{1} /\
+                 (o = 0 \/ o = 32){1} /\
+                 ={Glob.mem, o, k} /\ good_ptr output{1} plain{1} len{1} ==> ={Glob.mem}).
+    + proc.
+      while (={i,o,k,Glob.mem} /\ good_ptr output{1} plain{1} len{1} /\ 0 <= i{1} /\
+             output{1} = to_uint output{2} /\ 512 <= len{1} /\ (o = 0 \/ o = 32){1}).
+      + wp;skip => /> *;split;2:smt().
+        have h : to_uint (W64.of_int (o{2} + 64 * i{2})) = o{2} + 64 * i{2}.
+        + by apply W64.to_uint_small => /= /#.
+        by rewrite W64.to_uintD_small h /= /#.
+      wp; while (={i,o,k,Glob.mem} /\ good_ptr output{1} plain{1} len{1} /\ 0 <= i{1} /\
+             plain{1} = to_uint plain{2} /\ 512 <= len{1} /\ (o = 0 \/ o = 32){1}). 
+      + wp; skip=> /> *; split; 2:smt().
+        have h : to_uint (W64.of_int (o{2} + 64 * i{2})) = o{2} + 64 * i{2}.
+        + by apply W64.to_uint_small => /= /#.
+        by rewrite W64.to_uintD_small h /= /#.
+      by wp; skip => />.
+    + by move=> />; rewrite hout hplain hlen ho.
+    done.
+  byphoare (_:    disj_or_eq output plain len
+               /\ k = half_x8_ k1 k2 k3 k4 k5 k6 k7 k8
+               /\ (o0 = 0 \/ o0 = 32)
+               /\ output = output0
+               /\ plain = plain0
+               /\ o = o0
+               /\ len = len0
+               /\ 512 <= len
+               /\ Glob.mem = mem0 
+             ==>
+               !forall j, Glob.mem.[j] =
+                  upd_mem
+                  (mapi 0 (xor_mem_half o0 mem0 output0 plain0)
+                  [k1; k2; k3; k4; k5; k6; k7; k8]) mem0 output0 j) => //.
+  by hoare; conseq (pavx2_half_store_x8_spec mem0 k1 k2 k3 k4 k5 k6 k7 k8 output0 plain0 len0 o0).
+qed.
+
+lemma W8u32_bits128_0 (w:W8u32.Pack.pack_t) :
+  pack8_t w \bits128 0 = pack4 [w.[0]; w.[1]; w.[2]; w.[3]].
+proof. by rewrite -{1}(W8u32.Pack.to_listK w) /= -pack2_4u32_8u32. qed.
+
+lemma W8u32_bits128_1 (w:W8u32.Pack.pack_t) :
+  pack8_t w \bits128 1 = pack4 [w.[4]; w.[5]; w.[6]; w.[7]].
+proof. by rewrite -{1}(W8u32.Pack.to_listK w) /= -pack2_4u32_8u32. qed.
+
+lemma W4u32_bits64_0 (w:W4u32.Pack.pack_t) :
+  pack4_t w \bits64 0 = pack2 [w.[0]; w.[1]].
+proof. by rewrite -{1}(W4u32.Pack.to_listK w) /= -pack2_2u32_4u32. qed.
+
+lemma W4u32_bits64_1 (w:W4u32.Pack.pack_t) :
+  pack4_t w \bits64 1 = pack2 [w.[2]; w.[3]].
+proof. by rewrite -{1}(W4u32.Pack.to_listK w) /= -pack2_2u32_4u32. qed.
+
+(*lemma W2u128_W8u32 (w:W2u128.Pack.pack_t) : 
+   pack2_t w = pack8 [w.[0] \bits32 0 ; w.[0] \bits32 1; w.[0] \bits32 2 ; w.[0] \bits32 3;
+                      w.[1] \bits32 0 ; w.[1] \bits32 1; w.[1] \bits32 2 ; w.[1] \bits32 3].
+proof.
+  rewrite -pack2_4u32_8u32; congr.
+  apply W2u128.Pack.all_eq_eq; rewrite /all_eq /=.
+  rewrite -{1}(W4u32.unpack32K w.[0]) -{1}(W4u32.unpack32K w.[1]).
+  by rewrite /unpack32;split;congr;rewrite W4u32.Pack.init_of_list.
+qed.*)
+
+hint simplify (W8u32_bits128_0, W8u32_bits128_1, W4u32_bits64_0, W4u32_bits64_1).
+
+lemma x86_VPUNPCKH_8u32_spec (v0 v1 v2 v3 v4 v5 v6 v7 : W32.t) 
+                             (w0 w1 w2 w3 w4 w5 w6 w7 : W32.t): 
+  x86_VPUNPCKH_8u32 (W8u32.pack8 [v0; v1; v2; v3; v4; v5; v6; v7])
+                    (W8u32.pack8 [w0; w1; w2; w3; w4; w5; w6; w7]) =
+  W8u32.pack8 [v2; w2; v3; w3; v6; w6; v7; w7].
+proof.
+  by cbv delta; rewrite -(pack2_4u32_8u32 v2); congr; apply W2u128.Pack.all_eq_eq; rewrite /all_eq.
+qed.
+
+lemma x86_VPUNPCKL_8u32_spec (v0 v1 v2 v3 v4 v5 v6 v7 : W32.t) 
+                             (w0 w1 w2 w3 w4 w5 w6 w7 : W32.t): 
+  x86_VPUNPCKL_8u32 (W8u32.pack8 [v0; v1; v2; v3; v4; v5; v6; v7])
+                    (W8u32.pack8 [w0; w1; w2; w3; w4; w5; w6; w7]) =
+  W8u32.pack8 [v0; w0; v1; w1; v4; w4; v5; w5].
+proof.
+  by cbv delta; rewrite -(pack2_4u32_8u32 v0 w0); congr; apply W2u128.Pack.all_eq_eq; rewrite /all_eq.
+qed.
+
+lemma x86_VPERM2I128_8u32_spec_32 (v0 v1 v2 v3 v4 v5 v6 v7 : W32.t) (w0 w1 w2 w3 w4 w5 w6 w7 : W32.t):
+  x86_VPERM2I128 (W8u32.pack8 [v0; v1; v2; v3; v4; v5; v6; v7]) (W8u32.pack8 [w0; w1; w2; w3; w4; w5; w6; w7]) (W8.of_int 32) =
+  W8u32.pack8 [v0; v1; v2; v3; w0; w1; w2; w3].
+proof.
+  by cbv delta; rewrite !of_intwE; cbv delta; rewrite pack2_4u32_8u32.
+qed.
+
+lemma x86_VPERM2I128_8u32_spec_49 (v0 v1 v2 v3 v4 v5 v6 v7 : W32.t) (w0 w1 w2 w3 w4 w5 w6 w7 : W32.t):
+  x86_VPERM2I128 (W8u32.pack8 [v0; v1; v2; v3; v4; v5; v6; v7]) (W8u32.pack8 [w0; w1; w2; w3; w4; w5; w6; w7]) (W8.of_int 49) =
+  W8u32.pack8 [v4; v5; v6; v7; w4; w5; w6; w7].
+proof.
+  by cbv delta; rewrite !of_intwE; cbv delta; rewrite pack2_4u32_8u32.
+qed.
+
+lemma x86_VPUNPCKL_4u64_8u32 (v0 v1 v2 v3 v4 v5 v6 v7 : W32.t) (w0 w1 w2 w3 w4 w5 w6 w7 : W32.t):
+  x86_VPUNPCKL_4u64 (W8u32.pack8 [v0; v1; v2; v3; v4; v5; v6; v7]) (W8u32.pack8 [w0; w1; w2; w3; w4; w5; w6; w7]) =
+  W8u32.pack8 [v0;v1;w0;w1;v4;v5;w4;w5].
+proof.
+  by cbv delta; rewrite W2u128.Pack.init_of_list /= !pack2_2u32_4u32 pack2_4u32_8u32 .
+qed.
+
+lemma x86_VPUNPCKH_4u64_8u32 (v0 v1 v2 v3 v4 v5 v6 v7 : W32.t) (w0 w1 w2 w3 w4 w5 w6 w7 : W32.t):
+  x86_VPUNPCKH_4u64 (W8u32.pack8 [v0; v1; v2; v3; v4; v5; v6; v7]) (W8u32.pack8 [w0; w1; w2; w3; w4; w5; w6; w7]) =
+  W8u32.pack8 [v2;v3;w2;w3;v6;v7;w6;w7].
+proof.
+  by cbv delta; rewrite W2u128.Pack.init_of_list /= !pack2_2u32_4u32 pack2_4u32_8u32 .
+qed.
+
+hint simplify (x86_VPUNPCKH_8u32_spec, x86_VPUNPCKL_8u32_spec, x86_VPERM2I128_8u32_spec_32, x86_VPERM2I128_8u32_spec_49,
+               x86_VPUNPCKL_4u64_8u32, x86_VPUNPCKH_4u64_8u32).
+
+hoare rotate_spec k1 k2 k3 k4 k5 k6 k7 k8 : ChaCha20_savx2.M.rotate :
+   x = half_x8 k1 k2 k3 k4 k5 k6 k7 k8 ==>
+   res = half_x8_ k1 k2 k3 k4 k5 k6 k7 k8.
+proof.
+  conseq (_: Array8.all_eq res (half_x8_ k1 k2 k3 k4 k5 k6 k7 k8)).
+  + by move=> *;apply Array8.all_eq_eq.
+  proc.
+  inline M.sub_rotate.
+  unroll for ^while.   
+  unroll for ^while.
+  wp; skip => &hr /= ->.
+  have -> : W8.of_int (1 %% 16 + 48) = W8.of_int 49 by cbv delta.
+  have -> : W8.of_int (0 %% 16 + 32) = W8.of_int 32 by cbv delta.
+  by rewrite /all_eq /half_x8 /half_x8_ /= .
+qed.
+
+hoare rotate_stack_spec k1 k2 k3 k4 k5 k6 k7 k8 : ChaCha20_savx2.M.rotate_stack :
+   s = half_x8 k1 k2 k3 k4 k5 k6 k7 k8 ==>
+   res = half_x8_ k1 k2 k3 k4 k5 k6 k7 k8.
+proof.
+  conseq (_: Array8.all_eq res (half_x8_ k1 k2 k3 k4 k5 k6 k7 k8)).
+  + by move=> *;apply Array8.all_eq_eq.
+  proc.
+  inline M.sub_rotate.
+  do 3!(unroll for ^while).   
+  wp; skip => &hr /= ->.
+  have -> : W8.of_int (1 %% 16 + 48) = W8.of_int 49 by cbv delta.
+  have -> : W8.of_int (0 %% 16 + 32) = W8.of_int 32 by cbv delta.
+  by rewrite /all_eq /half_x8 /half_x8_ /= .
+qed.
+
+phoare store_half_x8_ll : [ M.store_half_x8 : true ==> true] = 1%r.
+proof.
+  proc.
+  while true (8 - i); 1: by move=> z;auto => /#.
+  wp; while true (8 - i); 1: by move=> z;auto => /#.
+  by auto => /#.
+qed.
+
+phoare sub_rotate_ll : [ M.sub_rotate : true ==> true] = 1%r.   
+proof. by proc; while true (4 - i); auto => /#. qed.
+
+phoare rotate_stack_pspec k1 k2 k3 k4 k5 k6 k7 k8 : 
+  [ChaCha20_savx2.M.rotate_stack :
+   s = half_x8 k1 k2 k3 k4 k5 k6 k7 k8 ==>
+   res = half_x8_ k1 k2 k3 k4 k5 k6 k7 k8] = 1%r.
+proof.
+  conseq (_:true ==> true) (rotate_stack_spec k1 k2 k3 k4 k5 k6 k7 k8).
+  + done.
+  proc;do 2! unroll for ^while.
+  by call sub_rotate_ll;auto.
+qed.
+
+op sub8 i (k:'a Array16.t) = Array8.of_list witness (Array16.sub k i 8).
+
+hoare rotate_first_half_x8_spec k1 k2 k3 k4 k5 k6 k7 k8 : M.rotate_first_half_x8 : 
+   k = x8 k1 k2 k3 k4 k5 k6 k7 k8 ==>
+   res.`1 = half_x8_ (sub8 0 k1) (sub8 0 k2) (sub8 0 k3) (sub8 0 k4) (sub8 0 k5) (sub8 0 k6) (sub8 0 k7) (sub8 0 k8) /\
+   res.`2 = half_x8 (sub8 8 k1) (sub8 8 k2) (sub8 8 k3) (sub8 8 k4) (sub8 8 k5) (sub8 8 k6) (sub8 8 k7) (sub8 8 k8).
+proof.
+  proc.
+  ecall (rotate_spec (sub8 0 k1) (sub8 0 k2) (sub8 0 k3) (sub8 0 k4) (sub8 0 k5) (sub8 0 k6) (sub8 0 k7) (sub8 0 k8)).
+  while (0 <= i <= 8 /\ forall j, 0 <= j < i => k0_7.[j] = k.[j]).
+  + by wp; skip; smt (Array8.get_setE).
+  wp; while (0 <= i <= 8 /\ forall j, 0 <= j < i => s_k8_15.[j] = k.[8 + j]).
+  + by wp; skip; smt (Array8.get_setE).
+  wp; skip => />; split; 1:smt().
+  move=> i0 s_k8_15 ??? h1; split; 1:smt().
+  move=> i1 k0_7 ??? h2.
+  have ->> : i0 = 8 by smt().
+  have ->> : i1 = 8 by smt().
+  split; apply Array8.all_eq_eq; rewrite /Array8.all_eq /=.
+  + by rewrite !h2; cbv delta.
+  by rewrite !h1; cbv delta.
+qed.
+
+phoare rotate_first_half_x8_pspec k1 k2 k3 k4 k5 k6 k7 k8 : 
+  [M.rotate_first_half_x8 : 
+   k = x8 k1 k2 k3 k4 k5 k6 k7 k8 ==>
+   res.`1 = half_x8_ (sub8 0 k1) (sub8 0 k2) (sub8 0 k3) (sub8 0 k4) (sub8 0 k5) (sub8 0 k6) (sub8 0 k7) (sub8 0 k8) /\
+   res.`2 = half_x8 (sub8 8 k1) (sub8 8 k2) (sub8 8 k3) (sub8 8 k4) (sub8 8 k5) (sub8 8 k6) (sub8 8 k7) (sub8 8 k8)] = 1%r.
+proof.
+  conseq (_:true ==> true) (rotate_first_half_x8_spec k1 k2 k3 k4 k5 k6 k7 k8).
+  + done.
+  proc; inline M.rotate; wp.
+  call sub_rotate_ll.
+  by do 3! unroll for ^while;auto.
+qed.
+
+lemma sub8_second_half k j: 
+  32 <= j < 64 =>
+  (WArray32.init32 ("_.[_]" (sub8 8 k))).[j - 32] = (WArray64.init32 ("_.[_]" k)).[j].
+proof.
+  move=> h;rewrite /WArray32.init32 /WArray64.init32 !initiE /=.
+  + smt (). + smt().
+  rewrite /sub8 /= /Array16.sub /mkseq /=.
+  have -> : -32 = (-8) * 4 by done.
+  rewrite modzMDr divzMDr 1://;congr.
+  have hj1 : 8 <= j %/ 4 < 16.
+  + rewrite lez_divRL //= ltz_divLR //.
+  by rewrite  Array8.get_of_list /#.
+qed.
+
+lemma sub8_first_half k j: 
+  0 <= j < 32 =>
+  (WArray32.init32 ("_.[_]" (sub8 0 k))).[j] = (WArray64.init32 ("_.[_]" k)).[j].
+proof.
+  move=> h;rewrite /WArray32.init32 /WArray64.init32 !initiE /=.
+  + smt (). + smt().
+  rewrite /sub8 /= /Array16.sub /mkseq /=.
+  have hj1 : 0 <= j %/ 4 < 8.
+  + rewrite lez_divRL //= ltz_divLR //.
+  by rewrite  Array8.get_of_list /#.
+qed.
+
+lemma nth_mapi k (f: int -> 'a -> 'b) al dfl j : 
+  nth dfl (mapi k f al) j = 
+   if 0 <= j < size al then f (k+j) (nth witness al j) else dfl.
+proof. elim: al k j => /= [ /# | a al hrec k j]; smt(size_ge0). qed.
+
+lemma upd_mem_mapi_8 output (f : int -> W32.t Array8.t -> int -> W8.t) ks mem j: 
+   upd_mem (mapi 0 f ks) mem output j = 
+    if in_range output (64 * size ks) j then
+      f ((j - output) %/64) (nth witness ks ((j - output) %/64)) ((j-output) %% 64)
+    else mem.[j].
+proof. 
+  rewrite /upd_mem size_mapi; case: (in_range output (64 * size ks) j) => //= hin.
+  rewrite nth_mapi ltz_divLR 1:// lez_divRL 1:// /= /#.
+qed.
+
+lemma upd_mem_mapi_16 output (f : int -> W32.t Array16.t -> int -> W8.t) ks mem j: 
+   upd_mem (mapi 0 f ks) mem output j = 
+    if in_range output (64 * size ks) j then
+      f ((j - output) %/64) (nth witness ks ((j - output) %/64)) ((j-output) %% 64)
+    else mem.[j].
+proof. 
+  rewrite /upd_mem size_mapi; case: (in_range output (64 * size ks) j) => //= hin.
+  rewrite nth_mapi ltz_divLR 1:// lez_divRL 1:// /= /#.
+qed.
+
+lemma upd_mem_half_2 len (mem1 mem0 mem2:global_mem_t) output plain k1 k2 k3 k4 k5 k6 k7 k8:
+  disj_or_eq output plain len =>  512 <= len => 
+  (forall (j : address),
+      mem1.[j] =
+      upd_mem (mapi 0 (xor_mem_half 0 mem0 output plain)
+                 [sub8 0 k1; sub8 0 k2; sub8 0 k3; sub8 0 k4; sub8 0 k5; sub8 0 k6; sub8 0 k7; sub8 0 k8]) mem0 output j) =>
+  (forall (j : address),
+      mem2.[j] =
+      upd_mem (mapi 0 (xor_mem_half 32 mem1 output plain)
+                 [sub8 8 k1; sub8 8 k2; sub8 8 k3; sub8 8 k4; sub8 8 k5; sub8 8 k6; sub8 8 k7; sub8 8 k8]) mem1 output j) =>
+   (forall (j:address),
+      mem2.[j] = 
+         upd_mem (mapi 0 (xor_mem mem0 plain) [k1; k2; k3; k4; k5; k6; k7; k8]) mem0 output j).
+proof.
+  move=> hd hlen hmem1 hmem2 j.
+  rewrite upd_mem_mapi_16 hmem2 upd_mem_mapi_8.
+  have -> : [sub8 8 k1; sub8 8 k2; sub8 8 k3; sub8 8 k4; sub8 8 k5; sub8 8 k6; sub8 8 k7; sub8 8 k8] = 
+            map (sub8 8) [k1;k2;k3;k4;k5;k6;k7;k8] by done.
+  have heq : [sub8 0 k1; sub8 0 k2; sub8 0 k3; sub8 0 k4; sub8 0 k5; sub8 0 k6; sub8 0 k7; sub8 0 k8] = 
+            map (sub8 0) [k1;k2;k3;k4;k5;k6;k7;k8] by done.
+  have hs : size [k1; k2; k3; k4; k5; k6; k7; k8] = 8 by done.
+  rewrite size_map hs.
+  pose k := nth witness [k1; k2; k3; k4; k5; k6; k7; k8] ((j - output) %/ 64).
+  case _ : (in_range output (64 * 8) j) => /= hj;last first.
+  + by rewrite hmem1 /upd_mem size_mapi /= hj.
+  rewrite (nth_map witness witness (sub8 8) ((j - output) %/ 64) [k1;k2;k3;k4;k5;k6;k7;k8]).
+  + by rewrite lez_divRL 1:// ltz_divLR //= /#.
+  rewrite -/k /xor_mem_half /xor_mem.
+  case: (32 <= (j -output) %% 64 < 32 + 32) => h. 
+  + congr; 1: by apply sub8_second_half.
+    rewrite hmem1 upd_mem_mapi_8 heq size_map hs.
+    pose k' := (map (sub8 0) [k1; k2; k3; k4; k5; k6; k7; k8]).   
+    case: (in_range output (64 * 8) (plain + 64 * ((j - output) %/ 64) + (j - output) %% 64)) => [h1 | //].
+    have ->> : plain = output by smt(divz_eq).
+    have -> : output + 64 * ((j - output) %/ 64) + (j - output) %% 64 - output = 
+              (j - output) %% 64 + ((j - output) %/ 64) * 64 by ring.
+    rewrite modzMDr divzMDr 1:// modz_mod (divz_small ((j - output) %% 64)); 1:smt(modz_cmp).
+    rewrite /= /k' (nth_map witness witness (sub8 0)).
+    + by rewrite lez_divRL 1:// ltz_divLR //= /#.
+    rewrite -/k /xor_mem_half; smt(modz_cmp).
+  rewrite hmem1 upd_mem_mapi_8 heq size_map hs.
+  pose k' := (map (sub8 0) [k1; k2; k3; k4; k5; k6; k7; k8]). 
+  have -> /= : output + 64 * ((j - output) %/ 64) + (j - output) %% 64 = j by smt(divz_eq).  
+  rewrite hj /= /k' (nth_map witness witness (sub8 0)).
+  + by rewrite lez_divRL 1:// ltz_divLR //= /#.
+  rewrite -/k /xor_mem_half. 
+  have h1 :  0 <= (j - output) %% 64 < 0 + 32 by smt(modz_cmp).
+  by rewrite h1 /=; congr; rewrite sub8_first_half.
+qed.
+
+hoare savx2_store_x8_spec mem0 k1 k2 k3 k4 k5 k6 k7 k8 output0 plain0 len0:
+  ChaCha20_savx2.M.store_x8 : 
+    disj_or_eq output0 plain0 len0 /\ good_ptr output0 plain0 len0 /\
+    k = x8 k1 k2 k3 k4 k5 k6 k7 k8 /\ 
+    to_uint output = output0 /\ to_uint plain = plain0 /\ to_uint len = len0 /\ 512 <= len0 /\ Glob.mem = mem0 
+    ==>
+    to_uint res.`1 = output0 + 512 /\ to_uint res.`2 = plain0 + 512 /\ to_uint res.`3 = len0 - 512 /\
+    (forall j, 
+       Glob.mem.[j] =
+       upd_mem (mapi 0 (xor_mem mem0 plain0) [k1; k2; k3; k4; k5; k6; k7; k8]) mem0 output0 j).
+proof.
+  proc.
+  inline M.update_ptr;wp.
+  ecall (savx2_half_store_x8_spec Glob.mem{hr} (sub8 8 k1) (sub8 8 k2) (sub8 8 k3) (sub8 8 k4) (sub8 8 k5) (sub8 8 k6) (sub8 8 k7) (sub8 8 k8)
+            output0 plain0 len0 32).
+  inline M.rotate_second_half_x8;wp.
+  ecall (rotate_stack_spec (sub8 8 k1) (sub8 8 k2) (sub8 8 k3) (sub8 8 k4) (sub8 8 k5) (sub8 8 k6) (sub8 8 k7) (sub8 8 k8)).
+  wp.
+  ecall (savx2_half_store_x8_spec Glob.mem{hr} (sub8 0 k1) (sub8 0 k2) (sub8 0 k3) (sub8 0 k4) (sub8 0 k5) (sub8 0 k6) (sub8 0 k7) (sub8 0 k8)
+            output0 plain0 len0 0).
+  ecall (rotate_first_half_x8_spec k1 k2 k3 k4 k5 k6 k7 k8); wp; skip => /> &hr h1 h2 h3 h4 [r1 r2] /= ?? mem1 w1 mem2 w2.
+  rewrite !W64.to_uintD_small /= 1..2:/#.
+  rewrite W32.to_uintB 1:uleE 1:// /=.
+  by apply (upd_mem_half_2 (to_uint len{hr}) mem1 Glob.mem{hr} mem2 (to_uint output{hr}) (to_uint plain{hr}) k1 k2 k3 k4 k5 k6 k7 k8).
+qed.
+
+phoare savx2_store_x8 mem0 k1 k2 k3 k4 k5 k6 k7 k8 output0 plain0 len0:
+  [ChaCha20_savx2.M.store_x8 : 
+    disj_or_eq output0 plain0 len0 /\ good_ptr output0 plain0 len0 /\
+    k = x8 k1 k2 k3 k4 k5 k6 k7 k8 /\ 
+    to_uint output = output0 /\ to_uint plain = plain0 /\ to_uint len = len0 /\ 512 <= len0 /\ Glob.mem = mem0 
+    ==>
+    to_uint res.`1 = output0 + 512 /\ to_uint res.`2 = plain0 + 512 /\ to_uint res.`3 = len0 - 512 /\
+    (forall j, 
+       Glob.mem.[j] =
+       upd_mem (mapi 0 (xor_mem mem0 plain0) [k1; k2; k3; k4; k5; k6; k7; k8]) mem0 output0 j)] = 1%r.
+proof.
+  conseq (_: true ==> true) (savx2_store_x8_spec mem0 k1 k2 k3 k4 k5 k6 k7 k8 output0 plain0 len0);1:done.
+  proc;  inline M.rotate_second_half_x8 M.rotate_first_half_x8 M.rotate M.rotate_stack.
+  call (_: true); 1: by auto.
+  call store_half_x8_ll; wp.
+  call sub_rotate_ll; wp.
+  while true (4 - i1); 1: by auto => /#.
+  wp; while true (4 - i1); 1: by auto => /#.
+  wp; call store_half_x8_ll; wp.
+  call sub_rotate_ll; wp.
+  wp; while true (4 - i0); 1: by auto => /#.
+  wp; while true (8 - i); 1: by auto => /#.
+  wp; while true (8 - i); auto => /#.
+qed.
+
+lemma upd_mem_comp (mem0 mem1 mem2:global_mem_t) output plain len ks (k:W32.t Array16.t) : 
+   inv_ptr output plain len =>
+   64 * size ks + 64 <= len =>
+   let ofs = 64 * size ks in
+   (forall j, mem1.[j] = upd_mem (mapi 0 (xor_mem mem0 plain) ks) mem0 output j) =>
+   (forall j, mem2.[j] = 
+         if in_range (output + ofs) 64 j then
+            (WArray64.init32 (fun (i0 : int) => k.[i0])).[j - (output + ofs)] `^`
+             mem1.[plain + ofs + (j - (output + ofs))]
+         else mem1.[j]) =>
+   forall j, mem2.[j] = upd_mem (mapi 0 (xor_mem mem0 plain) (rcons ks k)) mem0 output j.
+proof.
+  move=> /= hinv hlen hmem1 hupd j.
+  rewrite mapi_rcons upd_mem_rcons hupd size_mapi !hmem1.
+  case: (in_range (output + 64 * size ks) 64 j) => [hj | //].
+  rewrite /upd_mem /= size_mapi /xor_mem.
+  have -> /= : !in_range output (64 * size ks) (plain + 64 * size ks + (j - (output + 64 * size ks))) by smt (size_ge0).
+  have -> // : j - (output + 64*size ks) = (j - output) %% 64.
+  have -> : j - output = j - (output + 64*size ks) + size ks * 64 by ring.
+  by rewrite modzMDr modz_small /#.  
+qed.
+  
+phoare pref_store_ll : [ChaCha20_pref.M.store : true ==> true] = 1%r.
+proof.
+  proc;inline *;wp.
+  while true (min 64 len -i).
+  + by move=> z; wp; skip => /#.
+  wp; while true (min 64 len -i).
+  + by move=> z; wp; skip => /#.
+  by wp; skip => /#.  
+qed.
+
+phoare pavx2_store_x8_spec mem0 k1 k2 k3 k4 k5 k6 k7 k8 output0 plain0 len0:
+  [ ChaCha20_pavx2_cf.M.store_x8 : 
+    inv_ptr output plain len /\
+    k_1 = k1 /\ k_2 = k2 /\ k_3 = k3 /\ k_4 = k4 /\ k_5 = k5 /\ k_6 = k6 /\ k_7 = k7 /\ k_8 = k8 /\
+    output = output0 /\ plain = plain0 /\ len = len0 /\ 512 <= len /\ Glob.mem = mem0 
+    ==>
+    res = (output0 + 512, plain0 + 512, len0 - 512) /\
+    (forall j, 
+       Glob.mem.[j] =
+       upd_mem (mapi 0 (xor_mem mem0 plain0) [k1; k2; k3; k4; k5; k6; k7; k8]) mem0 output0 j)] = 1%r.
+proof.
+  conseq  (_: true ==> true) (_: 
+    inv_ptr output plain len /\
+    k_1 = k1 /\ k_2 = k2 /\ k_3 = k3 /\ k_4 = k4 /\ k_5 = k5 /\ k_6 = k6 /\ k_7 = k7 /\ k_8 = k8 /\
+    output = output0 /\ plain = plain0 /\ len = len0 /\ 512 <= len /\ Glob.mem = mem0 
+    ==>
+    res = (output0 + 512, plain0 + 512, len0 - 512) /\
+    (forall j, 
+       Glob.mem.[j] =
+       upd_mem (mapi 0 (xor_mem mem0 plain0) [k1; k2; k3; k4; k5; k6; k7; k8]) mem0 output0 j)); last first.
+  + by proc; do 8!call pref_store_ll; skip.
+  + by move=> />.
+  proc => /=.
+  ecall (store64_spec output{hr} plain{hr} len{hr} k8 Glob.mem{hr}).
+  ecall (store64_spec output{hr} plain{hr} len{hr} k7 Glob.mem{hr}).
+  ecall (store64_spec output{hr} plain{hr} len{hr} k6 Glob.mem{hr}).
+  ecall (store64_spec output{hr} plain{hr} len{hr} k5 Glob.mem{hr}).
+  ecall (store64_spec output{hr} plain{hr} len{hr} k4 Glob.mem{hr}).
+  ecall (store64_spec output{hr} plain{hr} len{hr} k3 Glob.mem{hr}).
+  ecall (store64_spec output{hr} plain{hr} len{hr} k2 Glob.mem{hr}).
+  ecall (store64_spec output{hr} plain{hr} len{hr} k1 Glob.mem{hr}).
+  skip. move=> &hr [#] hinv 11!->> ? ->> /= />.
+  split; [smt() | move=> h1 h2 {h1 h2} mem1 hinv1 hmem1].
+  split; [smt() | move=> h {h} mem2 hinv2 hmem2].
+  split; [smt() | move=> h {h} mem3 hinv3 hmem3].
+  split; [smt() | move=> h {h} mem4 hinv4 hmem4].
+  split; [smt() | move=> h {h} mem5 hinv5 hmem5].
+  split; [smt() | move=> h {h} mem6 hinv6 hmem6].
+  split; [smt() | move=> h {h} mem7 hinv7 hmem7].
+  split; [smt() | move=> h {h} mem8 hinv8 hmem8].
+  have hup1 := upd_mem_comp mem0 mem0 mem1 output0 plain0 len0 [] k1 hinv _ _ hmem1.
+  + smt(). + by move=> j /=; rewrite /upd_mem /= (_:!in_range output0 0 j) 1:/#.
+  have hup2 := upd_mem_comp mem0 mem1 mem2 output0 plain0 len0 [k1] k2 hinv _ hup1 hmem2; 1: by smt().
+  have hup3 := upd_mem_comp mem0 mem2 mem3 output0 plain0 len0 [k1;k2] k3 hinv _ hup2 hmem3; 1: by smt().
+  have hup4 := upd_mem_comp mem0 mem3 mem4 output0 plain0 len0 [k1;k2;k3] k4 hinv _ hup3 hmem4; 1: by smt().
+  have hup5 := upd_mem_comp mem0 mem4 mem5 output0 plain0 len0 [k1;k2;k3;k4] k5 hinv _ hup4 hmem5; 1: by smt().
+  have hup6 := upd_mem_comp mem0 mem5 mem6 output0 plain0 len0 [k1;k2;k3;k4;k5] k6 hinv _ hup5 hmem6; 1: by smt().
+  have hup7 := upd_mem_comp mem0 mem6 mem7 output0 plain0 len0 [k1;k2;k3;k4;k5;k6] k7 hinv _ hup6 hmem7; 1: by smt().
+  by apply (upd_mem_comp mem0 mem7 mem8 output0 plain0 len0 [k1;k2;k3;k4;k5;k6;k7] k8 hinv _ hup7 hmem8); smt().
+qed.
+
+equiv eq_store_x8 : ChaCha20_pavx2_cf.M.store_x8 ~  M.store_x8 :
+  k{2} = (x8 k_1 k_2 k_3 k_4 k_5 k_6 k_7 k_8){1} /\ 
+  output{1} = to_uint output{2} /\ plain{1} = to_uint plain{2} /\ len{1} = to_uint len{2} /\
+  (good_ptr output plain len){1} /\ disj_or_eq output{1} plain{1} len{1} /\ 512 <= len{1} /\
+  ={Glob.mem} 
+  ==>
+  res{1}.`1 = to_uint res{2}.`1 /\ res{1}.`2 = to_uint res{2}.`2 /\ res{1}.`3 = to_uint res{2}.`3 /\ 
+  (good_ptr res{1}.`1 res{1}.`2 res{1}.`3){1} /\ (disj_or_eq res{1}.`1 res{1}.`2 res{1}.`3){1} /\
+  ={Glob.mem}.
+proof.
+  proc *.
+  ecall{1} (pavx2_store_x8_spec Glob.mem{1} k_1{1} k_2{1} k_3{1} k_4{1} k_5{1} k_6{1} k_7{1} k_8{1} output{1} plain{1} len{1}).
+  ecall{2} (savx2_store_x8 Glob.mem{1} k_1{1} k_2{1} k_3{1} k_4{1} k_5{1} k_6{1} k_7{1} k_8{1} output{1} plain{1} len{1}).
+  skip => |> &1 &2 _ 3!-> hg hd hlen /= [r1 r2 r3] mem1 /= 3!-> hmem1; split; 1:smt().
+  move=> _ mem2 hmem2 /=;split; [smt() | split;1:smt()].
+  by apply Jasmin_memory.mem_eq_ext => j;rewrite hmem1 hmem2.
+qed.
+
+op x4_ (k1 k2 k3 k4:W32.t Array16.t) = 
+  Array8.of_list witness [
+    W8u32.pack8 [k1.[0]; k1.[1]; k1.[2]; k1.[3]; k1.[4]; k1.[5]; k1.[6]; k1.[7]];
+    W8u32.pack8 [k1.[8]; k1.[9]; k1.[10]; k1.[11]; k1.[12]; k1.[13]; k1.[14]; k1.[15]];
+    W8u32.pack8 [k2.[0]; k2.[1]; k2.[2]; k2.[3]; k2.[4]; k2.[5]; k2.[6]; k2.[7]];
+    W8u32.pack8 [k2.[8]; k2.[9]; k2.[10]; k2.[11]; k2.[12]; k2.[13]; k2.[14]; k2.[15]];
+    W8u32.pack8 [k3.[0]; k3.[1]; k3.[2]; k3.[3]; k3.[4]; k3.[5]; k3.[6]; k3.[7]];
+    W8u32.pack8 [k3.[8]; k3.[9]; k3.[10]; k3.[11]; k3.[12]; k3.[13]; k3.[14]; k3.[15]];
+    W8u32.pack8 [k4.[0]; k4.[1]; k4.[2]; k4.[3]; k4.[4]; k4.[5]; k4.[6]; k4.[7]];
+    W8u32.pack8 [k4.[8]; k4.[9]; k4.[10]; k4.[11]; k4.[12]; k4.[13]; k4.[14]; k4.[15]]
+ ].
+
+equiv eq_store_x4_last : ChaCha20_pavx2_cf.M.store_x4_last ~  M.store_x4_last :
+  k{2} = (x4_ k_1 k_2 k_3 k_4){1} /\
+  output{1} = to_uint output{2} /\ plain{1} = to_uint plain{2} /\ len{1} = to_uint len{2} /\
+  (good_ptr output plain len){1} /\ inv_ptr output{1} plain{1} len{1} /\ len{1} <= 256 /\
+  ={Glob.mem} 
+  ==>
+  ={Glob.mem}.
+proof.
+  proc => /=.
+  seq 0 3 : (#pre /\ (r.[0] = k.[0] /\ r.[1] = k.[1] /\ r.[2] = k.[2] /\ r.[3] = k.[3]){2}).
+  + by unroll for{2} ^while;wp; skip => />.
+  sp 2 0.
+  if.
+  + by move=> /> *; rewrite W32.uleE.
+  + call eq_store_x2_last => /=.
+    unroll for{2} ^while; wp.
+    ecall (eq_store_x2 len{1});skip => /> &1 &2 h1 h2 h3 hlen1 e0 e1 e2 e3 hlen2.
+    split. 
+    + by apply Array4.all_eq_eq;rewrite /all_eq /= /x2_ e0 e1 e2 e3 /x4_.  
+    move=> [r1 r2 r3] /> re -> ???;split; 1:smt().
+    by apply Array4.all_eq_eq;rewrite /all_eq /= /x4_ /= /x2_ /=.
+  call eq_store_x2_last; skip => /> &1 &2 h1 h2 h3 hlen1 e0 e1 e2 e3 hlen2.
+  split; 1:smt(). 
+  by apply Array4.all_eq_eq;rewrite /all_eq /= /x2_ e0 e1 e2 e3 /x4_.
+qed.
+
+phoare pavx2_store_x4_spec mem0 k1 k2 k3 k4 output0 plain0 len0:
+  [ ChaCha20_pavx2_cf.M.store_x4 : 
+    inv_ptr output plain len /\
+    k_1 = k1 /\ k_2 = k2 /\ k_3 = k3 /\ k_4 = k4 /\
+    output = output0 /\ plain = plain0 /\ len = len0 /\ 256 <= len /\ Glob.mem = mem0 
+    ==>
+    res = (output0 + 256, plain0 + 256, len0 - 256) /\
+    (forall j, 
+       Glob.mem.[j] =
+       upd_mem (mapi 0 (xor_mem mem0 plain0) [k1; k2; k3; k4]) mem0 output0 j)] = 1%r.
+proof.
+  conseq  (_: true ==> true) (_: 
+    inv_ptr output plain len /\
+    k_1 = k1 /\ k_2 = k2 /\ k_3 = k3 /\ k_4 = k4 /\ 
+    output = output0 /\ plain = plain0 /\ len = len0 /\ 256 <= len /\ Glob.mem = mem0 
+    ==>
+    res = (output0 + 256, plain0 + 256, len0 - 256) /\
+    (forall j, 
+       Glob.mem.[j] =
+       upd_mem (mapi 0 (xor_mem mem0 plain0) [k1; k2; k3; k4]) mem0 output0 j)); last first.
+  + by proc; do 4!call pref_store_ll; skip.
+  + by move=> />.
+  proc => /=.
+  ecall (store64_spec output{hr} plain{hr} len{hr} k4 Glob.mem{hr}).
+  ecall (store64_spec output{hr} plain{hr} len{hr} k3 Glob.mem{hr}).
+  ecall (store64_spec output{hr} plain{hr} len{hr} k2 Glob.mem{hr}).
+  ecall (store64_spec output{hr} plain{hr} len{hr} k1 Glob.mem{hr}).
+  skip=> &hr [#] hinv 7!->> ? ->> /= />.
+  split; [smt() | move=> h1 h2 {h1 h2} mem1 hinv1 hmem1].
+  split; [smt() | move=> h {h} mem2 hinv2 hmem2].
+  split; [smt() | move=> h {h} mem3 hinv3 hmem3].
+  split; [smt() | move=> h {h} mem4 hinv4 hmem4].
+  have hup1 := upd_mem_comp mem0 mem0 mem1 output0 plain0 len0 [] k1 hinv _ _ hmem1.
+  + smt(). + by move=> j /=; rewrite /upd_mem /= (_:!in_range output0 0 j) 1:/#.
+  have hup2 := upd_mem_comp mem0 mem1 mem2 output0 plain0 len0 [k1] k2 hinv _ hup1 hmem2; 1: by smt().
+  have hup3 := upd_mem_comp mem0 mem2 mem3 output0 plain0 len0 [k1;k2] k3 hinv _ hup2 hmem3; 1: by smt().
+  by apply (upd_mem_comp mem0 mem3 mem4 output0 plain0 len0 [k1;k2;k3] k4 hinv _ hup3 hmem4); smt().
+qed.
+
+module Store_x4 = {
+  proc store_x4 (output:int, plain:int, len:int, k:W256.t Array8.t) : int * int * int = {
+    var i:int;
+    i <- 0;
+    while (i < 8) {
+      k.[i] <- k.[i] `^` loadW256 Glob.mem (plain + 32 * i);
+      i <- i + 1;
+    }
+    i <- 0;
+    while (i < 8) {
+      Glob.mem <- storeW256 Glob.mem (output + (32 * i)) k.[i];
+      i <- i + 1;
+    }
+    (output, plain, len) <@ ChaCha20_pref.M.update_ptr (output, plain, len, 256);
+    return (output, plain, len);
+  }
+}.
+
+lemma storeW256_upd_mem (mem0 mem1:global_mem_t) ks output plain (k1:W32.t Array16.t):
+  (forall j, mem1.[j] = upd_mem ks mem0 output j) =>
+  (forall j,
+      (storeW256
+         (storeW256 
+            mem1 (output + 64 * size ks)
+            (pack8 [k1.[0]; k1.[1]; k1.[2]; k1.[3]; k1.[4]; k1.[5]; k1.[6]; k1.[7]] `^`
+                   loadW256 mem0 (plain + 64 * size ks)))
+         (output + 64 * size ks + 32)
+         (pack8 [k1.[8]; k1.[9]; k1.[10]; k1.[11]; k1.[12]; k1.[13]; k1.[14]; k1.[15]] `^`
+                      loadW256 mem0 (plain + 64 * size ks + 32))).[j] = 
+          upd_mem (rcons ks (xor_mem mem0 plain (size ks) k1)) mem0 output j).
+proof.
+  move=> hmem1 j.
+  rewrite !get_storeW256E.
+  have := store_256_xor_spec (output + 64 * size ks) k1 mem0 (plain + 64 * size ks) j.
+  rewrite upd_mem_rcons.
+  case: (in_range (output + 64 * size ks) 64 j) => hj; last by smt().
+  rewrite /xor_mem.
+  have -> /# : (j - output) %% 64 = j - (output + 64 * size ks).
+  have -> : j - output = j - (output + 64 * size ks) + size ks * 64 by ring.
+  by rewrite modzMDr modz_small /#.
+qed.
+
+phoare Store_x4_spec mem0 k1 k2 k3 k4 output0 plain0 len0:
+  [Store_x4.store_x4 : 
+    k = x4_ k1 k2 k3 k4 /\ 
+    output = output0 /\ plain = plain0 /\ len = len0 /\ 256 <= len0 /\ Glob.mem = mem0 
+    ==>
+    res = (output0 + 256, plain0 + 256, len0 - 256) /\
+    (forall j, 
+       Glob.mem.[j] =
+       upd_mem (mapi 0 (xor_mem mem0 plain0) [k1; k2; k3; k4]) mem0 output0 j)] = 1%r.
+proof.
+  conseq (_ : true ==> true)
+    (_ : k = x4_ k1 k2 k3 k4 /\ 
+    output = output0 /\ plain = plain0 /\ len = len0 /\ 256 <= len0 /\ Glob.mem = mem0 
+    ==>
+    res = (output0 + 256, plain0 + 256, len0 - 256) /\
+    (forall j, 
+       Glob.mem.[j] =
+       upd_mem (mapi 0 (xor_mem mem0 plain0) [k1; k2; k3; k4]) mem0 output0 j)).
+  + done. 
+  + proc => /=.
+    inline ChaCha20_pref.M.update_ptr;wp.
+    do 2! unroll for ^while;wp;skip => /> &hr (* hinv *) hlen j.
+    rewrite /x4_ /=.
+    have hmem1 := storeW256_upd_mem Glob.mem{hr} Glob.mem{hr} [] output{hr} plain{hr} k1 _; 1: by smt().
+    have {hmem1} hmem2 := storeW256_upd_mem Glob.mem{hr} _ _ output{hr} plain{hr} k2 hmem1.
+    have {hmem2} hmem3 := storeW256_upd_mem Glob.mem{hr} _ _ output{hr} plain{hr} k3 hmem2.
+    by apply (storeW256_upd_mem Glob.mem{hr} _ _ output{hr} plain{hr} k4 hmem3).
+  by proc; inline *; do 2!unroll for ^while;wp;skip.
+qed.
+
+equiv eq_store_x4 len0 : ChaCha20_pavx2_cf.M.store_x4 ~ M.store_x4 :
+  output{1} = to_uint output{2} /\ plain{1} = to_uint plain{2} /\ len{1} = to_uint len{2} /\ len{1} = len0 /\
+  ={Glob.mem} /\
+  (good_ptr output plain len){1} /\ (inv_ptr output plain len){1} /\ 256 <= len{1} /\
+  k{2} = (x4_ k_1 k_2 k_3 k_4){1} 
+  ==>
+  res{1}.`1 = to_uint res{2}.`1 /\ res{1}.`2 = to_uint res{2}.`2 /\ res{1}.`3 = to_uint res{2}.`3 /\ 
+  res{1}.`3 = len0 - 256 /\
+  (good_ptr res{1}.`1 res{1}.`2 res{1}.`3){1} /\ (inv_ptr res{1}.`1 res{1}.`2 res{1}.`3){1} /\ ={Glob.mem}.
+proof.
+  exlim output{1}, plain{1} => output0 plain0.
+  transitivity Store_x4.store_x4 
+    (={Glob.mem, output, plain, len} /\ k{2} = (x4_ k_1 k_2 k_3 k_4){1} /\ 256 <= len{1} /\
+      (output = output0 /\ plain = plain0 /\ len = len0){1} /\
+      (good_ptr output plain len){1} /\ (inv_ptr output plain len){1}
+     ==> 
+       ={Glob.mem, res} /\ res{1} = (output0 + 256, plain0 + 256, len0 - 256) /\
+      (good_ptr res{1}.`1 res{1}.`2 res{1}.`3){1} /\ (inv_ptr res{1}.`1 res{1}.`2 res{1}.`3){1})
+    (={Glob.mem, k} /\ 
+       output{1} = to_uint output{2} /\ plain{1} = to_uint plain{2} /\ len{1} = to_uint len{2} /\ 
+       (good_ptr output plain len){1} /\ (inv_ptr output plain len){1} /\ 256 <= len{1} ==>
+     res{1}.`1 = to_uint res{2}.`1 /\ res{1}.`2 = to_uint res{2}.`2 /\ res{1}.`3 = to_uint res{2}.`3 /\ 
+     ={Glob.mem}).
+  + by move=> /> *; exists Glob.mem{2} (output, plain, len, x4_ k_1 k_2 k_3 k_4){1}; rewrite H6 => />.
+  + done. 
+  + proc *.
+    ecall{1} (pavx2_store_x4_spec Glob.mem{1} k_1{1} k_2{1} k_3{1} k_4{1} output0 plain0 len0).
+    ecall{2} (Store_x4_spec Glob.mem{1} k_1{1} k_2{1} k_3{1} k_4{1} output0 plain0 len0).
+    skip => /> &1 &2 3!-> /= ?????? mem1 hmem1 mem2 hmem2; split;2: smt().
+    by apply Jasmin_memory.mem_eq_ext => j;rewrite hmem1 hmem2.
+  proc => /=.
+  inline ChaCha20_pref.M.update_ptr  M.update_ptr; wp.
+  while (={i,Glob.mem, k} /\ output{1} = to_uint output{2} /\ (good_ptr output plain len){1} /\ 0 <= i{1} /\ 256 <= len{1}).
+  + wp; skip => /> &1 &2 h1 h2 h3 h4 h5;split;2:smt(); congr.
+    have heq : to_uint (W64.of_int (32 * i{2})) = 32 * i{2}.
+    + by rewrite W64.to_uint_small /= /#.
+    by rewrite to_uintD_small heq 2:// /#.
+  wp; while (={i,Glob.mem, k} /\ plain{1} = to_uint plain{2} /\ (good_ptr output plain len){1} /\ 0 <= i{1} /\ 256 <= len{1}).
+  + wp; skip => /> &1 &2 h1 h2 h3 h4 h5;split;2:smt(); congr.
+    have heq : to_uint (W64.of_int (32 * i{2})) = 32 * i{2}.
+    + by rewrite W64.to_uint_small /= /#.
+    by rewrite to_uintD_small heq 2:// /#.
+  wp; skip => /> *.
+  rewrite to_uintB 1:uleE 1:// !to_uintD_small //= 1,2:/#.
+qed.
+
+phoare interleave_0_spec s0 k0 o0 : 
+  [M.interleave_0 : s = s0 /\ k = k0 /\ o = o0 ==>
+    res = Array8.of_list witness [s0.[o0 + 0];k0.[o0 + 0]; s0.[o0 + 1];k0.[o0 + 1]; s0.[o0 + 2];k0.[o0 + 2]; s0.[o0 + 3];k0.[o0 + 3]]] = 1%r.
+proof.
+  proc => /=.
+  conseq (_: Array8.all_eq sk 
+              (Array8.of_list witness [s0.[o0]; k0.[o0]; s0.[o0 + 1]; k0.[o0 + 1]; s0.[o0 + 2]; k0.[o0 + 2]; s0.[o0 + 3]; k0.[o0 + 3]])).
+  + by move=> *;rewrite (Array8.ext_eq_all sk).
+  by unroll for ^while;wp;skip.
+qed.
+
+equiv eq_store_x8_last : ChaCha20_pavx2_cf.M.store_x8_last ~  M.store_x8_last :
+  k{2} = (x8 k_1 k_2 k_3 k_4 k_5 k_6 k_7 k_8){1} /\
+  output{1} = to_uint output{2} /\ plain{1} = to_uint plain{2} /\ len{1} = to_uint len{2} /\
+  len{1} <= 512 /\
+  (good_ptr output plain len){1} /\ disj_or_eq output{1} plain{1} len{1} /\ 
+  ={Glob.mem} 
+  ==>
+  ={Glob.mem}.
+proof.
+  proc => /=.
+  call eq_store_x4_last => /=.
+  conseq |>.
+  seq 4 9 : 
+    ( s_k0_7{2} = (half_x8_ (sub8 0 k_1) (sub8 0 k_2) (sub8 0 k_3) (sub8 0 k_4) (sub8 0 k_5) (sub8 0 k_6) (sub8 0 k_7) (sub8 0 k_8)){1} /\
+      k8_15{2} = (half_x8_ (sub8 8 k_1) (sub8 8 k_2) (sub8 8 k_3) (sub8 8 k_4) (sub8 8 k_5) (sub8 8 k_6) (sub8 8 k_7) (sub8 8 k_8)){1} /\
+    i0_7{2} = x4_ r_1{1} r_2{1} r_3{1} r_4{1} /\
+    output{1} = to_uint output{2} /\
+    plain{1} = to_uint plain{2} /\
+    len{1} = to_uint len{2} /\ len{1} <= 512 /\
+    good_ptr output{1} plain{1} len{1} /\ inv_ptr output{1} plain{1} len{1} /\ len{1} <= 512 /\ ={Glob.mem}).
+  + wp.
+    ecall{2} (interleave_0_spec s_k0_7{2} k8_15{2} 0) => /=.
+    inline M.rotate_second_half_x8;wp.
+    ecall{2} (rotate_stack_pspec (sub8 8 k_1{1}) (sub8 8 k_2{1}) (sub8 8 k_3{1}) (sub8 8 k_4{1}) 
+                                 (sub8 8 k_5{1}) (sub8 8 k_6{1}) (sub8 8 k_7{1}) (sub8 8 k_8{1}));wp.
+    ecall{2} (rotate_first_half_x8_pspec k_1{1} k_2{1} k_3{1} k_4{1} k_5{1} k_6{1} k_7{1} k_8{1});wp;skip => />.
+    move=> &1 &2 h1 h2 h3 h4 [s k] /= -> _;split;2:smt().
+    by cbv delta.
+  if.
+  + by move=> />;rewrite uleE /=.
+  + wp; ecall{2} (interleave_0_spec s_k0_7{2} k8_15{2} 4) => /=.
+    ecall (eq_store_x4 len{1}); skip => />.
+    move=> &1 &2 h1 h2 h3 h4 h5 [output1 plain1 len1] [output2 plain2 len2] /> h6 h7 h8 h9;split;2:smt().
+    by cbv delta.
+  skip => /> /#.
+qed.
+
+equiv eq_sum_states_x8 : ChaCha20_pavx2.M.sum_states_x8 ~ M.sum_states_x8 :
+  k{2} = (x8 k1 k2 k3 k4 k5 k6 k7 k8){1} /\
+  st{2} = (x8 st1 st2 st3 st4 st5 st6 st7 st8){1} 
+  ==>
+  res{2} = x8 res{1}.`1 res{1}.`2 res{1}.`3 res{1}.`4 res{1}.`5 res{1}.`6 res{1}.`7 res{1}.`8.
+proof.
+  proc => /=.
+  inline *.
+  transitivity*{1} { 
+    i <- 0;
+    while (i < 16) {
+      k1.[i] <- k1.[i] + st1.[i];
+      k2.[i] <- k2.[i] + st2.[i];
+      k3.[i] <- k3.[i] + st3.[i];
+      k4.[i] <- k4.[i] + st4.[i];
+      k5.[i] <- k5.[i] + st5.[i];
+      k6.[i] <- k6.[i] + st6.[i];
+      k7.[i] <- k7.[i] + st7.[i];
+      k8.[i] <- k8.[i] + st8.[i];
+      i <- i + 1;
+    }
+  }. + smt(). + done.
+  + by do 8! unroll for{1} ^while; unroll for{2} ^while; wp; skip => />.
+  while (={i} /\ #pre /\ 0 <= i{1}); 2: by auto.
+  wp; skip => /> &1 &2 ??; split; 2:smt().
+  by rewrite !get_x8 1,2:// -set_x8 1:// /x86_VPADD_8u32.
+qed.
+
+equiv eq_chacha20_more_than_256 : 
+  ChaCha20_pavx2.M.chacha20_more_than_256 ~ ChaCha20_savx2.M.chacha20_more_than_256 : 
+  output{1} = to_uint output{2} /\ plain{1} = to_uint plain{2} /\ len{1} = to_uint len{2} /\
+  key{1} = to_uint key{2} /\ nonce{1} = to_uint nonce{2} /\ ={counter,Glob.mem} /\
+  (key + 32 < W64.modulus /\ nonce + 12 < W64.modulus){1} /\
+  (good_ptr output plain len){1} /\ (disj_or_eq output plain len){1} 
+  ==>
+  ={Glob.mem}.
+proof.
+  proc => /=.
+  seq 1 4 : (s_r16{2} = g_r16 /\ s_r8{2} = g_r8 /\ st{2} = (x8 st1 st2 st3 st4 st5 st6 st7 st8){1} /\
+            output{1} = to_uint output{2} /\ plain{1} = to_uint plain{2} /\ len{1} = to_uint len{2} /\
+            (good_ptr output plain len){1} /\ (disj_or_eq output plain len){1} /\ ={Glob.mem}).
+  + call eq_init_x8; inline{2} M.load_shufb_cmd; wp; skip => />.
+  seq 1 1 : (#pre /\ len{1} <= 512).
+  + while (#pre). 
+    + call eq_increment_counter_x8 => /=.
+      call eq_store_x8 => /=.
+      call eq_sum_states_x8 => /=.   
+      call eq_rounds_x8 => /=. 
+      by inline M.copy_state_x8; wp; skip => |> &2 hg hd hl _ [r11 ri2 r13] [r21 r22 r23] /= 3!->> _ _;rewrite uleE.
+    by skip => |> *; rewrite uleE /#.
+  if; last by done.
+  + by move=> /> *; rewrite ultE.
+  call eq_store_x8_last.
+  call eq_sum_states_x8 => /=.   
+  call eq_rounds_x8 => /=. 
+  by inline M.copy_state_x8; wp; skip => />.
 qed.
 
 equiv eq_chacha20_avx2 : 
